{
 "cells": [
  {
   "cell_type": "markdown",
   "id": "567adfd4-96b7-4619-af40-83b896a78ea8",
   "metadata": {
    "jp-MarkdownHeadingCollapsed": true
   },
   "source": [
    "# Binomial Expansion and Sums of Higher Powers\n",
    "\n",
    "We want to find a way to calculate higher powers of $k^n$\n",
    "\n",
    "But how do we do it?\n",
    "\n",
    "We can try to find a way to calculate higher powers by basing them on lower powers of $k^n$, such that we can slowly but surely build every new power sum from scratch\n",
    "- But how do we link $k^n$ to previous sums $k^{n-1}$, $k^{n-2}$, $k^{n-3}$ etc...?\n",
    "\n",
    "Thinking back, there is actually a series that contains all the powers of `k`, know as the binomial expansion:\n",
    "\n",
    "$$\n",
    "(k + d)^{n} = \n",
    "\\dbinom{n}{0}k^{n}d^{0} + \n",
    "\\dbinom{n}{1}k^{n-1}d^{1} + \n",
    "\\dbinom{n}{2}k^{n-2}d^{2} + \n",
    "\\cdots + \n",
    "\\dbinom{n}{n-2}k^{2}d^{n-2} + \n",
    "\\dbinom{n}{n-1}k^{1}d^{n-1} + \n",
    "\\dbinom{n}{n}k^{0}d^{n}\n",
    "$$\n",
    "\n",
    "But the second term, `d`, still exists. Is there a way to make sure only `k` exist in this expansion?\n",
    "- What kind of base would cause powers of `d` to disappear but not affect the `k` terms?\n",
    "- If it were `0`, then it would eliminate every term\n",
    "- If it were `1`, it would keep the `k` term, and we can get rid of the `d` terms because they would not affect the `k` terms!\n",
    "\n",
    "$$\n",
    "(k + 1)^{n} = \n",
    "\\dbinom{n}{0}k^{n}1^{0} + \n",
    "\\dbinom{n}{1}k^{n-1}1^{1} + \n",
    "\\dbinom{n}{2}k^{n-2}1^{2} + \n",
    "\\cdots + \n",
    "\\dbinom{n}{n-2}k^{2}1^{n-2} + \n",
    "\\dbinom{n}{n-1}k^{1}1^{n-1} + \n",
    "\\dbinom{n}{n}k^{0}1^{n}\n",
    "$$\n",
    "\n",
    "With the power of `1`s removed, is equivalent to\n",
    "\n",
    "$$\n",
    "(k + 1)^{n} =\n",
    "\\dbinom{n}{0}k^{n} + \n",
    "\\dbinom{n}{1}k^{n-1} + \n",
    "\\dbinom{n}{2}k^{n-2} + \n",
    "\\cdots + \n",
    "\\dbinom{n}{n-2}k^{2} + \n",
    "\\dbinom{n}{n-1}k^{1} + \n",
    "\\dbinom{n}{n}k^{0}\n",
    "$$\n",
    "\n",
    "Further simplify the combinations, plus a few minor touchups\n",
    "\n",
    "$$\n",
    "(k + 1)^{n} = \n",
    "k^{n} + \n",
    "nk^{n-1} + \n",
    "\\dbinom{n}{2}k^{n-2} + \n",
    "\\cdots + \n",
    "\\dbinom{n}{n-2}k^{2} + \n",
    "nk + 1\n",
    "$$\n",
    "\n",
    "> Note that the binomial expansion is symmetric around $\\dfrac{n+1}{2}$, where $\\dbinom{n}{m} = \\dbinom{n}{n-m}$\n",
    "\n",
    "Wow! Now that we have an expression that contains $k^{n}$ and its previous powers, maybe we can start here?"
   ]
  },
  {
   "cell_type": "markdown",
   "id": "e9fbae42-4eb0-4b97-951b-d0e1ffeeb1d5",
   "metadata": {},
   "source": [
    "# Telescoping Sums and Sums of Higher Powers\n",
    "\n",
    "But wait, it also contains its next power, if we were to isolate $k^{n}$ directly\n",
    "\n",
    "$$\n",
    "k^{n} = \n",
    "(k + 1)^{n} -\n",
    "nk^{n-1} - \n",
    "\\dbinom{n}{2}k^{n-2} - \n",
    "\\cdots - \n",
    "\\dbinom{n}{n-2}k^{2} - \n",
    "nk - \n",
    "1\n",
    "$$\n",
    "\n",
    "And apply the summation, from `1` to `m`:\n",
    "\n",
    "$$\n",
    "\\sum_{k=1}^m k^{n} = \n",
    "\\sum_{k=1}^m (k + 1)^{n} - \n",
    "n \\sum_{k=1}^m k^{n-1} - \n",
    "\\dbinom{n}{2} \\sum_{k=1}^m k^{n-2} - \n",
    "\\cdots - \n",
    "\\dbinom{n}{n-2} \\sum_{k=1}^m k^{2} - \n",
    "n \\sum_{k=1}^m k - \n",
    "\\sum_{k=1}^m 1\n",
    "$$\n",
    "\n",
    "Then we see that we have to find the sum of the next power in order to find the sum of the current power\n",
    "\n",
    "$$\n",
    "\\textcolor{lightgray}{\\sum_{k=1}^m k^{n} =}\n",
    "\\sum_{k=1}^m (k + 1)^{n} \n",
    "\\textcolor{lightgray}{- \n",
    "    n \\sum_{k=1}^m k^{n-1} - \n",
    "    \\dbinom{n}{2} \\sum_{k=1}^m k^{n-2} - \n",
    "    \\cdots - \n",
    "    \\dbinom{n}{n-2} \\sum_{k=1}^m k^{2} - \n",
    "    n \\sum_{k=1}^m k - \n",
    "    \\sum_{k=1}^m 1\n",
    "}\n",
    "$$\n",
    "\n",
    "- But that defeats the whole purpose of building-up from previous powers, if we already know what the next power is\n",
    "\n",
    "So what can we do to remove the need for the higher power?\n",
    "\n",
    "Notice that we have these 2 terms\n",
    "\n",
    "$$\n",
    "(k + 1)^{n} \\textcolor{lightgray}{=} \n",
    "k^{n} \n",
    "\\textcolor{lightgray}{+ \n",
    "    nk^{n-1} + \n",
    "    \\dbinom{n}{2}k^{n-2} + \n",
    "    \\cdots + \n",
    "    \\dbinom{n}{n-2}k^{2} + \n",
    "    nk + 1\n",
    "}\n",
    "$$\n",
    "\n",
    "Thus if we take the sum of their difference, we will have a convergent result! And thus eliminates the problem of $(k+1)^n$\n",
    "\n",
    "Taking the sum of their difference\n",
    "\n",
    "$$\n",
    "\\sum_{k=1}^m (k + 1)^{n} - k^{n} = \n",
    "n \\sum_{k=1}^m k^{n-1} + \n",
    "\\dbinom{n}{2} \\sum_{k=1}^m k^{n-2} + \n",
    "\\cdots + \n",
    "\\dbinom{n}{n-2} \\sum_{k=1}^m k^{2} + \n",
    "n \\sum_{k=1}^m k + \n",
    "\\sum_{k=1}^m 1\n",
    "$$\n",
    "\n",
    "Focusing on this part\n",
    "\n",
    "$$\n",
    "\\sum_{k=1}^m (k + 1)^{n} - \n",
    "k^{n} \\textcolor{lightgray}{=\n",
    "    n \\sum_{k=1}^m k^{n-1} + \n",
    "    \\dbinom{n}{2} \\sum_{k=1}^m k^{n-2} + \n",
    "    \\cdots + \n",
    "    \\dbinom{n}{n-2} \\sum_{k=1}^m k^{2} + \n",
    "    n \\sum_{k=1}^m k + \n",
    "    \\sum_{k=1}^m 1\n",
    "}\n",
    "$$\n",
    "\n",
    "We have\n",
    "\n",
    "$$\n",
    "\\begin{align*}\n",
    "    \\sum_{k=1}^m (k + 1)^{n} - k^{n} &= \\cancel{2^{n}} - 1^{n} \\\\\n",
    "    & + \\cancel{3^{n}} - \\cancel{2^{n}} \\\\\n",
    "    & + \\space \\cdots - \\cancel{3^{n}} \\\\\n",
    "    & \\vdots \\\\\n",
    "    & + \\cancel{m^{n}} - \\cdots \\\\\n",
    "    & + (m+1)^{n} - \\cancel{m^{n}} \\\\\n",
    "    & \\\\\n",
    "    & = (m+1)^{n} - 1^{n} \\\\\n",
    "    & = (m+1)^{n} - 1\n",
    "\\end{align*}\n",
    "$$\n",
    "\n",
    "Thus\n",
    "\n",
    "$$\n",
    "\\sum_{k=1}^m (k + 1)^{n} - k^{n} = (m+1)^{n} - 1\n",
    "$$\n",
    "\n",
    "And\n",
    "\n",
    "$$\n",
    "(m+1)^{n} - 1 = \n",
    "n \\sum_{k=1}^m k^{n-1} + \n",
    "\\dbinom{n}{2} \\sum_{k=1}^m k^{n-2} + \n",
    "\\cdots + \n",
    "\\dbinom{n}{n-2} \\sum_{k=1}^m k^{2} + \n",
    "n \\sum_{k=1}^m k + \n",
    "\\sum_{k=1}^m 1\n",
    "$$\n",
    "\n",
    "We can simplify it a little bit\n",
    "\n",
    "$$\n",
    "(m+1)^{n} - 1 = \n",
    "n \\sum_{k=1}^m k^{n-1} + \n",
    "\\dbinom{n}{2} \\sum_{k=1}^m k^{n-2} + \n",
    "\\cdots + \n",
    "\\dbinom{n}{n-2} \\sum_{k=1}^m k^{2} + \n",
    "n \\sum_{k=1}^m k + \n",
    "m\n",
    "$$\n",
    "\n",
    "And then\n",
    "\n",
    "$$\n",
    "(m+1)^{n} - \n",
    "(m + 1) = \n",
    "n \\sum_{k=1}^m k^{n-1} + \n",
    "\\dbinom{n}{2} \\sum_{k=1}^m k^{n-2} + \n",
    "\\cdots + \n",
    "\\dbinom{n}{n-2} \\sum_{k=1}^m k^{2} + \n",
    "n \\sum_{k=1}^m k\n",
    "$$\n",
    "\n",
    "Wait a minute, but now we do not have any $k^n$ to work with, how are we going to find $k^n$?"
   ]
  },
  {
   "cell_type": "markdown",
   "id": "26ec6f8d-f276-4245-8da4-c37613ef92ff",
   "metadata": {},
   "source": [
    "# Correcting the Premise\n",
    "\n",
    "Let us go back to this part, before we did method of difference\n",
    "\n",
    "$$\n",
    "(k + 1)^{n} = \n",
    "\\dbinom{n}{0}k^{n} + \n",
    "\\dbinom{n}{1}k^{n-1} + \n",
    "\\dbinom{n}{2}k^{n-2} + \n",
    "\\cdots + \n",
    "\\dbinom{n}{n-2}k^{2} + \n",
    "\\dbinom{n}{n-1}k^{1} + \n",
    "\\dbinom{n}{n}k^{0}\n",
    "$$\n",
    "\n",
    "Notice as this is the closest expression left, to $k^n$, after we do telescoping sums\n",
    "\n",
    "$$\n",
    "\\textcolor{lightgray}{(k + 1)^{n} = \n",
    "    \\dbinom{n}{0}k^{n} +} \n",
    "\\dbinom{n}{1}k^{n-1} \n",
    "\\textcolor{lightgray}{+\n",
    "    \\dbinom{n}{2}k^{n-2} + \n",
    "    \\cdots + \n",
    "    \\dbinom{n}{n-2}k^{2} + \n",
    "    \\dbinom{n}{n-1}k^{1} + \n",
    "    \\dbinom{n}{n}k^{0}\n",
    "}\n",
    "$$\n",
    "\n",
    "Perhaps we can just make this $k^n$ from the start?\n",
    "\n",
    "---\n",
    "\n",
    "In order to do that we have to increase the power by `1` throughout, and adjust the coefficients accordingly\n",
    "\n",
    "\n",
    "Like so\n",
    "\n",
    "$$\n",
    "(k + 1)^{n+1} = \n",
    "\\dbinom{n+1}{0}k^{n+1} +\n",
    "\\dbinom{n+1}{1}k^{n} +\n",
    "\\dbinom{n+1}{2}k^{n-1} +\n",
    "\\cdots +\n",
    "\\dbinom{n+1}{n-1}k^{2} +\n",
    "\\dbinom{n+1}{n}k^{1} +\n",
    "\\dbinom{n+1}{n+1}k^{0}\n",
    "$$"
   ]
  },
  {
   "cell_type": "markdown",
   "id": "5a1d57ca-4b13-4e60-9845-32071a427282",
   "metadata": {},
   "source": [
    "# Going through the Steps\n",
    "\n",
    "And thus when we simplify\n",
    "\n",
    "$$\n",
    "\\textcolor{lightgray}{(k + 1)^{n+1} \n",
    "= \\space} \n",
    "k^{n+1} + \n",
    "(n+1)k^{n} + \n",
    "\\dbinom{n+1}{2}k^{n-1} + \n",
    "\\cdots + \n",
    "\\dbinom{n+1}{n-1}k^{2} + \n",
    "(n+1)k + 1\n",
    "$$\n",
    "\n",
    "And take the sum\n",
    "\n",
    "$$\n",
    "\\sum_{k=1}^m (k + 1)^{n+1} =\n",
    "\\sum_{k=1}^m k^{n+1} + \n",
    "(n+1) \\sum_{k=1}^m k^{n} + \n",
    "\\dbinom{n+1}{2} \\sum_{k=1}^m k^{n-1} + \n",
    "\\cdots + \n",
    "\\dbinom{n+1}{n-1} \\sum_{k=1}^m k^{2} + \n",
    "(n+1) \\sum_{k=1}^m k + \n",
    "\\sum_{k=1}^m 1\n",
    "$$\n",
    "\n",
    "And use the  method of differences\n",
    "\n",
    "$$\n",
    "\\sum_{k=1}^m (k + 1)^{n+1} - \n",
    "k^{n+1} \\textcolor{lightgray}{=\n",
    "(n+1) \\sum_{k=1}^m k^{n} + \n",
    "\\dbinom{n+1}{2} \\sum_{k=1}^m k^{n-1} + \n",
    "\\cdots + \n",
    "\\dbinom{n+1}{n-1} \\sum_{k=1}^m k^{2} + \n",
    "(n+1) \\sum_{k=1}^m k + \n",
    "\\sum_{k=1}^m 1}\n",
    "$$\n",
    "\n",
    "With the same logic we get this\n",
    "\n",
    "$$\n",
    "(m + 1)^{n+1} - 1 \\textcolor{lightgray}{= \n",
    "(n+1) \\sum_{k=1}^m k^{n} + \n",
    "\\dbinom{n+1}{2} \\sum_{k=1}^m k^{n-1} + \n",
    "\\cdots + \n",
    "\\dbinom{n+1}{n-1} \\sum_{k=1}^m k^{2} + \n",
    "(n+1) \\sum_{k=1}^m k + \n",
    "\\sum_{k=1}^m 1}\n",
    "$$\n",
    "\n",
    "With the same simplification on the sum of `1`\n",
    "\n",
    "$$\n",
    "\\textcolor{lightgray}{(m + 1)^{n+1} - 1 = \n",
    "(n+1) \\sum_{k=1}^m k^{n} + \n",
    "\\dbinom{n+1}{2} \\sum_{k=1}^m k^{n-1} + \n",
    "\\cdots + \n",
    "\\dbinom{n+1}{n-1} \\sum_{k=1}^m k^{2} + \n",
    "(n+1) \\sum_{k=1}^m k} + \n",
    "m\n",
    "$$\n",
    "\n",
    "Shift over\n",
    "\n",
    "$$\n",
    "(m + 1)^{n+1} - (m+1) \\textcolor{lightgray}{= \n",
    "(n+1) \\sum_{k=1}^m k^{n} + \n",
    "\\dbinom{n+1}{2} \\sum_{k=1}^m k^{n-1} + \n",
    "\\cdots + \n",
    "\\dbinom{n+1}{n-1} \\sum_{k=1}^m k^{2} + \n",
    "(n+1) \\sum_{k=1}^m k}\n",
    "$$\n",
    "\n",
    "We get to this\n",
    "\n",
    "$$\n",
    "(m + 1)^{n+1} - (m+1) = \n",
    "(n+1) \\sum_{k=1}^m k^{n} + \n",
    "\\dbinom{n+1}{2} \\sum_{k=1}^m k^{n-1} + \n",
    "\\cdots + \n",
    "\\dbinom{n+1}{n-1} \\sum_{k=1}^m k^{2} + \n",
    "(n+1) \\sum_{k=1}^m k\n",
    "$$\n",
    "\n",
    "Now that we can seek to isolate the term with $k^n$\n",
    "\n",
    "$$\n",
    "\\textcolor{lightgray}{(m + 1)^{n+1} - (m+1) =}\n",
    "(n+1) \\sum_{k=1}^m k^{n} \\textcolor{lightgray}{+ \n",
    "\\dbinom{n+1}{2} \\sum_{k=1}^m k^{n-1} + \n",
    "\\cdots + \n",
    "\\dbinom{n+1}{n-1} \\sum_{k=1}^m k^{2} + \n",
    "(n+1) \\sum_{k=1}^m k}\n",
    "$$\n",
    "\n",
    "Shift the rest of the summation over to the other side:\n",
    "\n",
    "$$\n",
    "\\textcolor{lightgray}{(n+1) \\sum_{k=1}^m k^{n}} =\n",
    "(m + 1)^{n+1} - (m+1) -\n",
    "\\dbinom{n+1}{2} \\sum_{k=1}^m k^{n-1} -\n",
    "\\cdots - \n",
    "\\dbinom{n+1}{n-1} \\sum_{k=1}^m k^{2} - \n",
    "(n+1) \\sum_{k=1}^m k\n",
    "$$\n",
    "\n",
    "Then shift the coefficient to the other side\n",
    "\n",
    "$$\n",
    "\\textcolor{lightgray}{\\sum_{k=1}^m k^{n}} = \n",
    "\\dfrac{1}{n+1} \n",
    "\\biggr[ (m + 1)^{n+1} - (m+1) - \n",
    "    \\dbinom{n+1}{2} \\sum_{k=1}^m k^{n-1} - \n",
    "    \\cdots - \n",
    "    \\dbinom{n+1}{n-1} \\sum_{k=1}^m k^{2} - \n",
    "    (n+1) \\sum_{k=1}^m k \n",
    "\\biggr]\n",
    "$$"
   ]
  },
  {
   "cell_type": "markdown",
   "id": "05b27e74-70af-4c90-bffa-792ac2282c24",
   "metadata": {},
   "source": [
    "# Recursive General Formula\n",
    "\n",
    "Thus we have arrived a general formula to build-up formulas for sums of higher powers, using binomial expansion and method of difference\n",
    "\n",
    "$$\n",
    "\\boxed{\n",
    "    \\sum_{k=1}^m k^{n} = \\dfrac{1}{n+1} \\biggr[ (m + 1)^{n+1} - (m+1) - \\dbinom{n+1}{2} \\sum_{k=1}^m k^{n-1} - \\cdots - \\dbinom{n+1}{n-1} \\sum_{k=1}^m k^{2} - (n+1) \\sum_{k=1}^m k \\biggr], \\quad \\text{for} \\space  n \\in \\mathbf Z^{+}\n",
    "    }\n",
    "$$\n",
    "\n",
    "- It will just be tedious, but it is proven possible to use this method to calculate all the sums of higher and higher integer powers\n",
    "\n",
    "But we can compress it even more\n",
    "\n",
    "---\n",
    "\n",
    "Notice this part has a pattern\n",
    "\n",
    "$$\n",
    "\\textcolor{lightgray}{\\sum_{k=1}^m k^{n} = \n",
    "\\dfrac{1}{n+1} \n",
    "\\biggr[ (m + 1)^{n+1} - \n",
    "    (m+1)} -\n",
    "    \\dbinom{n+1}{2} \\sum_{k=1}^m k^{n-1} -\n",
    "    \\cdots - \n",
    "    \\dbinom{n+1}{n-1} \\sum_{k=1}^m k^{2} - \n",
    "    (n+1) \\sum_{k=1}^m k \\textcolor{lightgray}\n",
    "{\\biggr], \\quad \\text{for n > 0}\n",
    "}\n",
    "$$\n",
    "\n",
    "When we revert it back into the form with clear combinations, we have\n",
    "\n",
    "$$\n",
    "\\textcolor{lightgray}{\\sum_{k=1}^m k^{n} = \n",
    "\\dfrac{1}{n+1} \n",
    "\\biggr[ (m + 1)^{n+1} - \n",
    "    (m+1)} -\n",
    "    \\dbinom{n+1}{2} \\sum_{k=1}^m k^{n-1} -\n",
    "    \\cdots - \n",
    "    \\dbinom{n+1}{n-1} \\sum_{k=1}^m k^{2} - \n",
    "    \\dbinom{n+1}{n} \\sum_{k=1}^m k \\textcolor{lightgray}\n",
    "{\\biggr], \\quad \\text{for n > 0}\n",
    "}\n",
    "$$\n",
    "\n",
    "The choice in combination notation increases from `2` to `n` \n",
    "\n",
    "$$\n",
    "\\textcolor{lightgray}{\\sum_{k=1}^m k^{n} = \n",
    "\\dfrac{1}{n+1} \n",
    "\\biggr[ (m + 1)^{n+1} - \n",
    "    (m+1)} \\textcolor{lightgray}{-}\n",
    "    \\dbinom{\\textcolor{lightgray}{n+1}}{2} \\textcolor{lightgray}{\\sum_{k=1}^m k^{n-1} -\n",
    "    \\cdots \\space -} \n",
    "    \\dbinom{\\textcolor{lightgray}{n+1}}{n-1} \\textcolor{lightgray}{\\sum_{k=1}^m k^{2} -} \n",
    "    \\dbinom{\\textcolor{lightgray}{n+1}}{n} \\textcolor{lightgray}{\\sum_{k=1}^m k \\biggr], \\quad \\text{for n > 0}\n",
    "}\n",
    "$$\n",
    "\n",
    "- Thus, we can contract all those sums, as sums of sums\n",
    "\n",
    "$$\n",
    "\\textcolor{lightgray}{\\sum_{k=1}^m k^n = \n",
    "    \\frac{1}{n+1} \\Biggl[ (m+1)^{n+1} - (m+1)} - \\sum_{j=2}^{n}  \\biggr[ \\binom{n+1}{j} \\sum_{k=1}^m k^{\\colorbox{lightgray}{\\quad}} \\biggr] \\textcolor{lightgray}{\\Biggr]}\n",
    "$$\n",
    "\n",
    "Now we need to figure out how the power of `k` relates to these sums\n",
    "\n",
    "We see that in the original, the power of `k` decreases from `n-1` to `1`\n",
    "\n",
    "$$\n",
    "\\textcolor{lightgray}{\\sum_{k=1}^m k^{n} = \n",
    "\\dfrac{1}{n+1} \n",
    "\\biggr[ (m + 1)^{n+1 - \n",
    "    (m+1)} -\n",
    "    \\dbinom{n+1}{2} \\sum_{k=1}^m} k^{n-1} \\textcolor{lightgray}{-\n",
    "    \\cdots - \n",
    "    \\dbinom{n+1}{n-1} \\sum_{k=1}^m} k^{2} \\textcolor{lightgray}{- \n",
    "    (n+1) \\sum_{k=1}^m} k \\textcolor{lightgray}\n",
    "{\\biggr], \\quad \\text{for n > 0}\n",
    "}\n",
    "$$\n",
    "\n",
    "While the choice in combination notation increases from `2` to `n`\n",
    "\n",
    "$$\n",
    "\\textcolor{lightgray}{\\sum_{k=1}^m k^{n} = \n",
    "\\dfrac{1}{n+1} \n",
    "\\biggr[ (m + 1)^{n+1} - \n",
    "    (m+1)} \\textcolor{lightgray}{-}\n",
    "    \\dbinom{\\textcolor{lightgray}{n+1}}{2} \\textcolor{lightgray}{\\sum_{k=1}^m k^{n-1} -\n",
    "    \\cdots \\space -} \n",
    "    \\dbinom{\\textcolor{lightgray}{n+1}}{n-1} \\textcolor{lightgray}{\\sum_{k=1}^m k^{2} -} \n",
    "    \\dbinom{\\textcolor{lightgray}{n+1}}{n} \\textcolor{lightgray}{\\sum_{k=1}^m k \\biggr], \\quad \\text{for n > 0}\n",
    "}\n",
    "$$\n",
    "\n",
    "- Now that the choice is represented by `j`, we see that for each of the power of `k`,\n",
    "- it is exactly `-j + 1` for the constant, and then `+n`\n",
    "- Giving us `-j + 1 + n`\n",
    "- Rearranged, such that the negative sign is not in front,\n",
    "- We have `n - j + 1` for the power of `k`\n",
    "\n",
    "$$\n",
    "\\textcolor{lightgray}{\\sum_{k=1}^m k^n = \n",
    "    \\frac{1}{n+1} \\Biggl[ (m+1)^{n+1} - (m+1)} - \\sum_{j=2}^{n}  \\biggr[ \\binom{n+1}{j} \\sum_{k=1}^m k^{n - j + 1} \\biggr] \\textcolor{lightgray}{\\Biggr]}\n",
    "$$\n",
    "\n",
    "---\n",
    "\n",
    "Thus, we get this compressed general formula of\n",
    "\n",
    "$$\n",
    "\\boxed{\n",
    "    \\sum_{k=1}^m k^n = \\frac{1}{n+1} \\left[ (m+1)^{n+1} - (m+1) - \\sum_{j=2}^{n}  \\biggr[ \\binom{n+1}{j} \\sum_{k=1}^m k^{n-j+1} \\biggr] \\right]\n",
    "}\n",
    "$$\n",
    "\n",
    "Which looks unneccessarily convoluted on the power of `k` because it is nested in another sum, when in fact it is just `1 less than n`, and `decreases by 1` down to `1`"
   ]
  }
 ],
 "metadata": {
  "kernelspec": {
   "display_name": "Python 3 (ipykernel)",
   "language": "python",
   "name": "python3"
  },
  "language_info": {
   "codemirror_mode": {
    "name": "ipython",
    "version": 3
   },
   "file_extension": ".py",
   "mimetype": "text/x-python",
   "name": "python",
   "nbconvert_exporter": "python",
   "pygments_lexer": "ipython3",
   "version": "3.12.9"
  }
 },
 "nbformat": 4,
 "nbformat_minor": 5
}
