{
 "cells": [
  {
   "cell_type": "markdown",
   "id": "b5bb6723-9b87-4c74-a999-0ff4f958cda2",
   "metadata": {},
   "source": [
    "## Sum of even numbers\n",
    "\n",
    "This is a pattern that emerged from the sum of even numbers\n",
    "$$\n",
    "\\begin{align}\n",
    "    0 &= 0 \\rightarrow 1 \\times 0 \\\\\n",
    "    2 &= 2 \\rightarrow 2 \\times 1 \\\\\n",
    "    2 + 4 &= 6 \\rightarrow 3 \\times 2 \\\\\n",
    "    2 + 4 + 6 &= 12 \\rightarrow 4 \\times 3 \\\\\n",
    "    2 + 4 + 6 + 8 &= 20 \\rightarrow 5 \\times 4 \\\\\n",
    "    2 + 4 + 6 + 8 + 10 &= 30 \\rightarrow 6 \\times 5 \\\\\n",
    "    2 + 4 + 6 + 8 + 10 + 12 &= 42 \\rightarrow 7 \\times 6 \\\\\n",
    "    2 + 4 + 6 + 8 + 10 + 12 + 14 &= 56 \\rightarrow 8 \\times 7 \\\\\n",
    "    2 + 4 + 6 + 8 + 10 + 12 + 14 + 16 &= 72 \\rightarrow 9 \\times 8 \\\\\n",
    "\\end{align}\n",
    "$$\n",
    "\n",
    "It seems that the sum of even numbers is the `current iteration` times its `previous iteration number`.\n",
    "\n",
    "But let's prove it!\n",
    "\n",
    "---\n",
    "\n",
    "We start from this:\n",
    "\n",
    "$$\n",
    "\\sum_{k=0}^n 2k\n",
    "$$\n",
    "\n",
    "Expand and Simplify\n",
    "\n",
    "We are going to use `0` to `n-1` here because...\n",
    "- ...the series I presented starts from `0`, which is the 1st iteration,\n",
    "- ...and to reach the `n`-th iteration, it will move another `n-1` steps, which lands us at `0 + n-1 = n-1`\n",
    "- ...which is why the last value for `k` is `n-1` instead of what we might mistake as `n`\n",
    "\n",
    "$$\n",
    "\\begin{align*}\n",
    "    \\sum_{k=0}^{n-1} 2k &= 2\\sum_{k=0}^{n-1} k \\\\\n",
    "    &= 2 \\space \\left( 0 + \\sum_{k=1}^{n-1} k \\right) \\\\\n",
    "    &= 2 \\sum_{k=1}^{n-1} k \\\\\n",
    "    &= \\cancel{2} \\cdot \\dfrac{(1 + (n-1))(n-1)}{\\cancel{2}} \\\\\n",
    "    &= n(n-1) \\\\\n",
    "\\end{align*}\n",
    "$$\n",
    "\n",
    "Thus we have proven this cool identity!\n",
    "\n",
    "$$\n",
    "\\underline{\n",
    "    \\sum_{k=0}^{n-1} 2k = n(n-1)\n",
    "}\n",
    "$$\n",
    "\n",
    "Notice although even numbers start from `0`, zero does not contribute to the sum, thus it is equivalent to starting from `1`\n",
    "- That fact is also present in our derivation step\n",
    "\n",
    "$$\n",
    "\\begin{align*}\n",
    "    \\textcolor{lightgray}{\\sum_{k=0}^{n-1} 2k} & \\textcolor{lightgray}{=} \\textcolor{lightgray}{2\\sum_{k=0}^{n-1} k} \\\\\n",
    "    & \\textcolor{lightgray}{=} \\textcolor{lightgray}{2} \\space \\left( 0 + \\sum_{k=1}^{n-1} k \\right) \\\\\n",
    "    & \\textcolor{lightgray}{\\vdots}\n",
    "\\end{align*}\n",
    "$$\n",
    "\n",
    "\n",
    "Thus\n",
    "\n",
    "$$\n",
    "\\boxed{\\sum_{k=1}^{n-1} 2k = n(n-1)}\n",
    "$$\n",
    "\n",
    "---\n",
    "\n",
    "The flipped multiplication, where the smaller number multiplies the bigger number is also true\n",
    "\n",
    "$$\n",
    "\\begin{align}\n",
    "    0 &= 0 \\rightarrow 0 \\times 1 \\\\\n",
    "    2 &= 2 \\rightarrow 1 \\times 2 \\\\\n",
    "    2 + 4 &= 6 \\rightarrow 2 \\times 3 \\\\\n",
    "    2 + 4 + 6 &= 12 \\rightarrow 3 \\times 4 \\\\\n",
    "    2 + 4 + 6 + 8 &= 20 \\rightarrow 4 \\times 5 \\\\\n",
    "    2 + 4 + 6 + 8 + 10 &= 30 \\rightarrow 5 \\times 6 \\\\\n",
    "    2 + 4 + 6 + 8 + 10 + 12 &= 42 \\rightarrow 6 \\times 7 \\\\\n",
    "    2 + 4 + 6 + 8 + 10 + 12 + 14 &= 56 \\rightarrow 7 \\times 8 \\\\\n",
    "    2 + 4 + 6 + 8 + 10 + 12 + 14 + 16 &= 72 \\rightarrow 8 \\times 9 \\\\\n",
    "\\end{align}\n",
    "$$\n",
    "\n",
    "So if we let it end at `k=n` instead of `k=n-1`\n",
    "\n",
    "$$\n",
    "\\begin{align*}\n",
    "    \\sum_{k=0}^{n} 2k &= 2\\sum_{k=0}^{n} k \\\\\n",
    "    &= 2 \\space \\left( 0 + \\sum_{k=1}^{n} k \\right) \\\\\n",
    "    &= 2 \\sum_{k=1}^{n} k \\\\\n",
    "    &= \\cancel{2} \\cdot \\dfrac{n(n+1)}{\\cancel{2}} \\\\\n",
    "    &= n(n+1) \\\\\n",
    "\\end{align*}\n",
    "$$\n",
    "\n",
    "Thus we have proven this cool identity in another perspective!\n",
    "\n",
    "$$\n",
    "\\underline{\\sum_{k=0}^{n} 2k = n(n+1)}\n",
    "$$\n",
    "\n",
    "With the same fact that zero does not contribute to the sum, we have this!\n",
    "\n",
    "$$\n",
    "\\boxed{\\sum_{k=1}^{n} 2k = n(n+1)}\n",
    "$$\n",
    "\n",
    "---\n",
    "\n",
    "Therefore!\n",
    "$$\n",
    "\\underline{\\sum_{k=0}^{n-1} 2k = n(n-1)} \\quad \\text{and} \\quad \\underline{\\sum_{k=0}^{n} 2k = n(n+1)}\n",
    "$$\n",
    "\n",
    "And thus!\n",
    "\n",
    "$$\n",
    "\\boxed{\\sum_{k=1}^{n-1} 2k = n(n-1)} \\quad \\text{and} \\quad \\boxed{\\sum_{k=1}^{n} 2k = n(n+1)}\n",
    "$$"
   ]
  }
 ],
 "metadata": {
  "kernelspec": {
   "display_name": "Python 3 (ipykernel)",
   "language": "python",
   "name": "python3"
  },
  "language_info": {
   "codemirror_mode": {
    "name": "ipython",
    "version": 3
   },
   "file_extension": ".py",
   "mimetype": "text/x-python",
   "name": "python",
   "nbconvert_exporter": "python",
   "pygments_lexer": "ipython3",
   "version": "3.12.9"
  }
 },
 "nbformat": 4,
 "nbformat_minor": 5
}
