{
 "cells": [
  {
   "cell_type": "markdown",
   "id": "4f28ee1f-add3-4f85-932c-4ffbebb58f9e",
   "metadata": {},
   "source": [
    "# Combinatorial Approach to the Sum of Cubes Formula\n",
    "\n",
    "We derive the formula for the sum of squares using a combinatorial approach by expressing the sum as a double summation, applying the arithmetic sequence formula, and then using algebraic manipulation.\n",
    "\n",
    "---\n",
    "Before Anything lets play with the sum a little\n",
    "\n",
    "## Algebraic Manipulation\n",
    "Let's seek to make the exponential into an addition problem\n",
    "$$\n",
    "\\sum_{k=1}^n k^3 = 1^3 + 2^3 + 3^3 + ... + n^3\n",
    "$$\n",
    "\n",
    "Re-write it in terms of multiplication\n",
    "$$\n",
    "\\sum_{k=1}^n k^3 = (1 \\cdot 1 \\cdot 1) + (2 \\cdot 2 \\cdot 2) + (3 \\cdot 3 \\cdot 3) + ... + (n \\cdot n \\cdot n)\n",
    "$$\n",
    "\n",
    "Re-write it in terms of addition\n",
    "$$\n",
    "\\begin{align*}\n",
    "\\sum_{k=1}^n k^3 &= 1 \\quad \\\\\n",
    "&\\quad + (2 + 2) + (2 + 2) \\quad \\\\\n",
    "&\\quad + (3 + 3 + 3) + (3 + 3 + 3) + (3 + 3 + 3) \\quad \\\\\n",
    "&\\quad \\vdots \\\\\n",
    "&\\quad + \\underbrace{(n + \\dots + n) + \\dots + (n + \\dots + n)}_{n \\text{ terms}}\n",
    "\\end{align*}\n",
    "$$\n",
    "\n",
    "Spot that vertically we have the sum of squares\n",
    "$$\n",
    "\\begin{align*}\n",
    "\\sum_{k=1}^n k^3 &= 1 + (2 + 2) + (3 + 3 + 3) + ... + (n + n + ... + n) \\quad \\\\\n",
    "&\\quad + (2 + 2) + (3 + 3 + 3) + ... + (n + n + ... + n) \\quad \\\\\n",
    "&\\quad + (3 + 3 + 3) + ... + (n + n + ... + n) \\quad \\\\\n",
    "&\\quad \\vdots \\\\\n",
    "&\\quad + (n + n + \\dots + n) \n",
    "\\end{align*}\n",
    "$$\n",
    "\n",
    "Therefore this is the sum of squares with an increasing starting point\n",
    "$$\n",
    "\\sum_{k=1}^n k^3 = \\left( \\sum_{j=1}^n j^2 + \\sum_{j=2}^n j^2 + \\sum_{j=3}^n j^2 + \\dots + \\sum_{j=n}^n j^2 \\right)\n",
    "$$\n",
    "\n",
    "Thus\n",
    "$$\n",
    "\\sum_{k=1}^n k^3 = \\underbrace{\\left( \\sum_{j=k}^n j^2 + \\sum_{j=k}^n j^2 + \\sum_{j=k}^n j^2 + \\dots + \\sum_{j=k}^n j^2 \\right)}_{\\text{For k from 1 to n}}\n",
    "$$\n",
    "\n",
    "This generalizes to:\n",
    "$$\n",
    "\\sum_{k=1}^n k^3 = \\sum_{k=1}^n \\left( \\sum_{j=k}^n j^2 \\right)\n",
    "$$\n",
    "\n",
    "Thus, we have a double summation\n",
    "$$\n",
    "\\boxed{\n",
    "    \\sum_{k=1}^n k^3 = \\sum_{k=1}^n \\sum_{j=k}^n j^2\n",
    "}\n",
    "$$"
   ]
  },
  {
   "cell_type": "markdown",
   "id": "df5529eb-772f-4f56-90aa-3ee71c7650cb",
   "metadata": {},
   "source": [
    "## Applying the sum of squares formula\n",
    "\n",
    "Lets isolate this:\n",
    "\n",
    "$$\n",
    "\\textcolor{darkgray}{\\sum_{k=1}^n k^3 = \\sum_{k=1}^n} \\sum_{j=k}^n j^2\n",
    "$$\n",
    "\n",
    "We know:\n",
    "\n",
    "$$\n",
    "\\sum_{j=1}^n j^2 = \\frac{n(n+1)(2n+1)}{6}\n",
    "$$\n",
    "\n",
    "The partial sum from $j=k$ to $j=n$ can be described like so:\n",
    "\n",
    "$$\n",
    "\\sum_{j=k}^n j^2 = \\sum_{j=1}^n j^2 - \\sum_{j=1}^{k-1} j^2\n",
    "$$\n",
    "\n",
    "Substituting the right variables we get:\n",
    "\n",
    "$$\n",
    "\\sum_{j=k}^n j^2 = \\frac{n(n+1)(2n+1)}{6} - \\frac{(k-1)k(2k-1)}{6}\n",
    "$$\n",
    "\n",
    "Thus, we have:\n",
    "\n",
    "$$\n",
    "\\sum_{k=1}^n k^3  = \\sum_{k=1}^n \\left( \\frac{n(n+1)(2n+1)}{6} - \\frac{(k-1)k(2k-1)}{6} \\right)\n",
    "$$"
   ]
  },
  {
   "cell_type": "markdown",
   "id": "69566f26-bb85-4ca0-b14b-6dea07059407",
   "metadata": {},
   "source": [
    "## Expand and Simplify\n",
    "Let \n",
    "\n",
    "$$\n",
    "\\mathbf{S_n} = \\sum_{k=1}^n k^3\n",
    "$$\n",
    "\n",
    "---\n",
    "\n",
    "Simplify the expression:\n",
    "\n",
    "$$\n",
    "\\mathbf{S_n} = \\frac{n^2(n+1)(2n+1)}{6} - \\frac{1}{6} \\sum_{k=1}^n (2k^3 - 3k^2 + k)\n",
    "$$\n",
    "\n",
    "$$\n",
    "6\\mathbf{S_n} = n^2(n+1)(2n+1) - \\sum_{k=1}^n (2k^3 - 3k^2 + k)\n",
    "$$\n",
    "\n",
    "Focusing on this term\n",
    "$$\n",
    "\\textcolor{lightgray}{6\\mathbf{S_n} = n^2(n+1)(2n+1)} \\textcolor{lightgray}{-} \\sum_{k=1}^n (2k^3 - 3k^2 + k)\n",
    "$$\n",
    "\n",
    "Distribute the summation\n",
    "\n",
    "$$\n",
    "\\sum_{k=1}^n (2k^3 - 3k^2 + k) = 2 \\left( \\sum_{k=1}^n k^3 \\right) - 3 \\left( \\sum_{k=1}^n k^2 \\right) + \\sum_{k=1}^n k\n",
    "$$\n",
    "\n",
    "This part is the sum we want to find\n",
    "\n",
    "$$\n",
    "2 \\left( \\sum_{k=1}^n k^3 \\right) \\textcolor{lightgray}{- 3 \\left( \\sum_{k=1}^n k^2 \\right) + \\sum_{k=1}^n k}\n",
    "$$\n",
    "\n",
    "$$\n",
    "2\\mathbf{S_n} \\textcolor{lightgray}{- 3 \\left( \\sum_{k=1}^n k^2 \\right) + \\sum_{k=1}^n k}\n",
    "$$\n",
    "\n",
    "This is the sum of squares\n",
    "$$\n",
    "\\textcolor{lightgray}{2\\mathbf{S_n}} - 3 \\left( \\sum_{k=1}^n k^2 \\right) + \\textcolor{lightgray}{\\sum_{k=1}^n k}\n",
    "$$\n",
    "\n",
    "$$\n",
    "\\textcolor{lightgray}{2\\mathbf{S_n}} - 3 \\cdot \\frac{n(n+1)(2n+1)}{6} + \\textcolor{lightgray}{\\sum_{k=1}^n k}\n",
    "$$\n",
    "\n",
    "$$\n",
    "\\textcolor{lightgray}{2\\mathbf{S_n}} - \\frac{n(n+1)(2n+1)}{2} + \\textcolor{lightgray}{\\sum_{k=1}^n k}\n",
    "$$\n",
    "\n",
    "This is the sum of arithmetic sequence\n",
    "\n",
    "$$\n",
    "\\textcolor{lightgray}{2\\mathbf{S_n} - \\frac{n(n+1)(2n+1)}{2}} + \\sum_{k=1}^n k\n",
    "$$\n",
    "\n",
    "$$\n",
    "\\textcolor{lightgray}{2\\mathbf{S_n} - \\frac{n(n+1)(2n+1)}{2}} + \\frac{n(n+1)}{2}\n",
    "$$\n",
    "\n",
    "Hence\n",
    "\n",
    "$$\n",
    "2\\mathbf{S_n} - \\frac{n(n+1)(2n+1)}{2} + \\frac{n(n+1)}{2}\n",
    "$$\n",
    "\n",
    "\n",
    "Simplify\n",
    "$$\n",
    "2\\mathbf{S_n} + \\frac{n(n+1)}{2} - \\frac{n(n+1)(2n+1)}{2} \n",
    "$$\n",
    "\n",
    "$$\n",
    "2\\mathbf{S_n} + \\frac{n(n+1)[1 - (2n + 1)]}{2}\n",
    "$$\n",
    "\n",
    "$$\n",
    "2\\mathbf{S_n} - \\frac{n(n+1)(\\cancel{2}n)}{\\cancel{2}}\n",
    "$$\n",
    "\n",
    "$$\n",
    "2\\mathbf{S_n} - n^2(n+1)\n",
    "$$\n",
    "\n",
    "Hence\n",
    "\n",
    "$$\n",
    "\\sum_{k=1}^n (2k^3 - 3k^2 + k) = 2\\mathbf{S_n} - n^2(n+1)\n",
    "$$\n",
    "\n",
    "---"
   ]
  },
  {
   "cell_type": "markdown",
   "id": "0eb6bc76-20a5-45d5-b498-afc6c30c19bd",
   "metadata": {},
   "source": [
    "Substitute back:\n",
    "$$\n",
    "\\textcolor{lightgray}{6\\mathbf{S_n} = n^2(n+1)(2n+1)} \\textcolor{lightgray}{-} \\sum_{k=1}^n (2k^3 - 3k^2 + k)\n",
    "$$\n",
    "\n",
    "$$\n",
    "6\\mathbf{S_n} = n^2(n+1)(2n+1) - \\left[ 2\\mathbf{S_n} - n^2(n+1) \\right]\n",
    "$$\n",
    "\n",
    "Distribute the signs:\n",
    "\n",
    "$$\n",
    "6\\mathbf{S_n} = n^2(n+1)(2n+1) - 2\\mathbf{S_n} + n^2(n+1)\n",
    "$$\n",
    "\n",
    "Shift $S_n$ over\n",
    "$$\n",
    "8\\mathbf{S_n} = n^2(n+1)(2n+1) + n^2(n+1)\n",
    "$$\n",
    "\n",
    "Combine like terms:\n",
    "\n",
    "$$\n",
    "8\\mathbf{S_n} = n^2(n+1)(2n+2)\n",
    "$$\n",
    "\n",
    "Simplify:\n",
    "$$\n",
    "8\\mathbf{S_n} = 2n^2(n+1)(n+1)\n",
    "$$\n",
    "\n",
    "$$\n",
    "4\\mathbf{S_n} = n^2(n+1)^2\n",
    "$$\n",
    "\n",
    "$$\n",
    "2^{2}\\mathbf{S_n} = n^2(n+1)^2\n",
    "$$\n",
    "\n",
    "$$\n",
    "\\mathbf{S_n} = \\frac{n^2(n+1)^2}{2^2}\n",
    "$$\n",
    "\n",
    "$$\n",
    "\\mathbf{S_n} = \\left[ \\frac{n(n+1)}{2} \\right]^2\n",
    "$$\n",
    "\n",
    "---\n",
    "\n",
    "## Final Result\n",
    "$$\n",
    "\\boxed{\\sum_{k=1}^n k^3 = \\left[ \\frac{n(n+1)}{2} \\right]^2}\n",
    "$$"
   ]
  },
  {
   "cell_type": "markdown",
   "id": "bd81bebe-cfb0-4c2c-a6d2-73ac9400bbce",
   "metadata": {},
   "source": [
    "## Explore Other Methods (Comprehensive Understanding)\n",
    "\n",
    "To deepen understanding, explore alternative methods:\n",
    "- **Mathematical Induction**: Prove the formula by assuming it holds for $n$ and showing it holds for $n+1$.\n",
    "    - This is a verification approach\n",
    "- **Telescoping Series**: Use $(k+1)^4 - k^4 = 4k^3 + 6k^2 + 4k + 1$ to derive the sum.\n",
    "    - This is a top-down derivation approach\n",
    "\n",
    "This comprehensive approach ensures a holistic grasp of the concept."
   ]
  }
 ],
 "metadata": {
  "kernelspec": {
   "display_name": "Python 3 (ipykernel)",
   "language": "python",
   "name": "python3"
  },
  "language_info": {
   "codemirror_mode": {
    "name": "ipython",
    "version": 3
   },
   "file_extension": ".py",
   "mimetype": "text/x-python",
   "name": "python",
   "nbconvert_exporter": "python",
   "pygments_lexer": "ipython3",
   "version": "3.12.9"
  }
 },
 "nbformat": 4,
 "nbformat_minor": 5
}
