{
 "cells": [
  {
   "cell_type": "markdown",
   "id": "e2fa3a67-5cdb-422b-9eed-dd6cb3357485",
   "metadata": {},
   "source": [
    "# Combinatorial Derivation of Sum of Cubes via Vertical Grouping\n",
    "\n",
    "## Initial Setup\n",
    "We start with the sum of cubes:\n",
    "$$\n",
    "\\sum_{k=1}^n k^3 = 1^3 + 2^3 + \\cdots + n^3\n",
    "$$\n",
    "\n",
    "## Step 1: Expand Cubes as Repeated Addition\n",
    "Each cube term can be expanded vertically:\n",
    "$$\n",
    "\\begin{align*}\n",
    "1^3 &= 1 \\\\\n",
    "2^3 &= (2 + 2) + (2 + 2) \\\\\n",
    "3^3 &= (3 + 3 + 3) + (3 + 3 + 3) + (3 + 3 + 3) \\\\\n",
    "&\\vdots \\\\\n",
    "n^3 &= \\underbrace{\\underbrace{(n + \\cdots + n)}_{n \\text{ times}} + \\cdots + {(n + \\cdots + n)}}_{n \\text{ times}}\n",
    "\\end{align*}\n",
    "$$\n",
    "\n",
    "Notice for the first row, we have $1$ of $1$\n",
    "- for the 2nd row, we have $2^2$ of $2$\n",
    "- for the 3rd row, we have $3^2$ of $3$\n",
    "- ...\n",
    "- This will continue for $n$ rows\n",
    "- for the nth row, we have $n^2$ of $n$\n",
    "\n",
    "This makes sense because\n",
    "\n",
    "$$\n",
    "\\begin{align}\n",
    "    n^3 &= n^2 \\cdot n \\\\\n",
    "    &= n \\cdot n^2 \\\\\n",
    "    &= n \\text{ of } n^2 \\\\\n",
    "\\end{align}\n",
    "$$\n",
    "\n",
    "Hence\n",
    "\n",
    "$$\n",
    "\\text{Number of } n^2 \\text{ is } \\boxed{n}\n",
    "$$\n"
   ]
  },
  {
   "cell_type": "markdown",
   "id": "b05bcbfe-09d5-4348-9aac-3412535ac89f",
   "metadata": {},
   "source": [
    "## Step 2: Observe Grouping Pattern\n",
    "\n",
    "List out the individual terms that add up to each term in the series\n",
    "\n",
    "$$\n",
    "\\begin{array}{c|ccccccccccc}\n",
    "    1^3 & 1 \\\\\n",
    "    2^3 & 2 & 2 & 2 & 2 \\\\\n",
    "    3^3 & 3 & 3 & 3 & 3 & 3 & 3 & 3 & 3 & 3 \\\\\n",
    "    \\vdots & \\vdots & \\vdots & \\vdots & \\vdots & \\vdots & \\vdots & \\vdots & \\vdots & \\vdots & \\ddots\\\\\n",
    "    n^3 & n & n & n & n & n & n & n & n & n & \\cdots & n\\\\\n",
    "\\end{array}\n",
    "$$\n",
    "\n",
    "By grouping vertically we have\n",
    "\n",
    "$$\n",
    "\\begin{array}{c|c:c:c:c:c:c:c:c:c:cc}\n",
    "    1^3 & 1 \\\\\n",
    "    2^3 & 2 & 2 & 2 & 2 \\\\\n",
    "    3^3 & 3 & 3 & 3 & 3 & 3 & 3 & 3 & 3 & 3 \\\\\n",
    "    \\vdots & \\vdots & \\vdots & \\vdots & \\vdots & \\vdots & \\vdots & \\vdots & \\vdots & \\vdots & \\ddots\\\\\n",
    "    n^3 & n & n & n & n & n & n & n & n & n & \\cdots & n\\\\\n",
    "\\end{array}\n",
    "$$\n",
    "\n",
    "Separate the groups by starting term\n",
    "\n",
    "$$\n",
    "\\begin{array}{c|c:ccc:ccccc:cc}\n",
    "    1^3 & 1 \\\\\n",
    "    2^3 & 2 & 2 & 2 & 2 \\\\\n",
    "    3^3 & 3 & 3 & 3 & 3 & 3 & 3 & 3 & 3 & 3 \\\\\n",
    "    \\vdots & \\vdots & \\vdots & \\vdots & \\vdots & \\vdots & \\vdots & \\vdots & \\vdots & \\vdots & \\ddots\\\\\n",
    "    n^3 & n & n & n & n & n & n & n & n & n & \\cdots & n\\\\\n",
    "\\end{array}\n",
    "$$\n",
    "\n",
    "And we have:\n",
    "\n",
    "$$\n",
    "\\begin{align*}\n",
    "    \\sum_{k=1}^n k^3 &= 1 \\cdot (1 + 2 + \\cdots + n) \\\\\n",
    "    &+ 3 \\cdot (2 + \\cdots + n) \\\\\n",
    "    &+ 5 \\cdot (3 + \\cdots + n) \\\\\n",
    "    &\\vdots \\\\\n",
    "    &+ \\,(2k-1) \\cdot (n) \\,?\\\\\n",
    "\\end{align*}\n",
    "$$\n",
    "\n",
    "It seems that this sum has odd weighted multipliers `e.g. 1, 3, 5`\n",
    "\n",
    "But let's verify it\n"
   ]
  },
  {
   "cell_type": "markdown",
   "id": "a3819a25-6e37-4ad6-a29b-8678da84a1b0",
   "metadata": {},
   "source": [
    "## Step 3: Verify the pattern\n",
    "We know that the number of each sequence starting from some number `k` is\n",
    "\n",
    "$$\n",
    "\\begin{align*}\n",
    "    &\\boxed{\\text{Number of raw current sequence: that starts from }k \\text{ of the k-th term}} - \\boxed{\\text{That of the previous sequence: } k-1} \\\\\n",
    "    &= \\boxed{k^2 \\textcolor{gray}{\\text{ of } k}} - \\boxed{(k-1)^2 \\textcolor{gray}{\\text{ of } (k-1)}} \\\\\n",
    "    &= k^2 - (k-1)^2\n",
    "\\end{align*}\n",
    "$$\n",
    "\n",
    "Let's expand and simplify that\n",
    "\n",
    "$$\n",
    "\\begin{align*}\n",
    "    &  k^2 - (k-1)^2 \\\\\n",
    "    &= k^2 - (k^2 - 2k + 1) \\\\\n",
    "    &= \\cancel{k^2} - \\cancel{k^2} + 2k - 1 \\\\\n",
    "    &= 2k - 1\n",
    "\\end{align*}\n",
    "$$\n",
    "\n",
    "Wow! So the difference of squares is also the odd number at that point!\n",
    "\n",
    "$$\n",
    "\\boxed{\n",
    "    \\begin{align*}\n",
    "    &\\text{Difference of squares} \\\\\n",
    "    &= \\text{Odd number} \n",
    "\\end{align*}\n",
    "}\n",
    "$$\n",
    "\n",
    "Thus we can affirm that\n",
    "\n",
    "$$\n",
    "\\begin{align*}\n",
    "    \\sum_{k=1}^n k^3 &= 1 \\cdot (1 + 2 + 3 + \\cdots + n) \\\\\n",
    "    &+ 3 \\cdot (2 + 3 +\\cdots + n)\\\\\n",
    "    &+ 5 \\cdot (3 + \\cdots + n) \\\\\n",
    "    &\\vdots \\\\\n",
    "    &+ (2k - 1)(n) \\\\\n",
    "\\end{align*}\n",
    "$$\n",
    "\n",
    "Thus in summation terms:\n",
    "\n",
    "$$\n",
    "\\begin{align*}\n",
    "    \\sum_{k=1}^n k^3 &= 1 \\cdot \\sum_{j=1}^n j + 3 \\cdot \\sum_{j=2}^n j + 5 \\cdot \\sum_{j=3}^n j + \\cdots + (2k - 1) \\sum_{j=k}^n j \\\\\n",
    "    &= \\underbrace{(2k - 1) \\sum_{j=k}^n j + (2k - 1) \\sum_{j=k}^n j + (2k - 1) \\sum_{j=k}^n j + \\cdots + (2k - 1) \\sum_{j=k}^n j}_{\\text{k from 1 to n}} \\\\\n",
    "    &= \\sum_{k=1}^n \\left[ (2k - 1) \\sum_{j=k}^n j \\right]\n",
    "\\end{align*}\n",
    "$$\n",
    "\n",
    "## Conclusion\n",
    "$$\n",
    "\\boxed{\n",
    "    \\sum_{k=1}^n k^3 = \\sum_{k=1}^n \\left[ (2k - 1) \\sum_{j=k}^n j \\right]\n",
    "}\n",
    "$$"
   ]
  },
  {
   "cell_type": "markdown",
   "id": "5d2226aa-d79a-46ad-bef9-091c12d5980d",
   "metadata": {},
   "source": [
    "# Derivation of Sum of Cubes from Double-Sum Identity\n",
    "\n",
    "## Given Identity\n",
    "$$\n",
    "\\sum_{k=1}^n k^3 = \\sum_{k=1}^n \\left[ (2k - 1) \\sum_{j=k}^n j \\right]\n",
    "$$\n",
    "\n",
    "## Step 1: Simplify Inner Sum\n",
    "Look at the inner sum\n",
    "\n",
    "$$\n",
    "\\textcolor{lightgray}{\\sum_{k=1}^n k^3 = \\sum_{k=1}^n} \\left[ \\textcolor{lightgray}{(2k - 1)} \\sum_{j=k}^n j \\right]\n",
    "$$\n",
    "\n",
    "We can derive the general form of the sum of squares by removing a part from the whole\n",
    "\n",
    "$$\n",
    "\\begin{align}\n",
    "    \\sum_{j=k}^n j &= \\sum_{j=1}^n j - \\sum_{j=1}^{k-1} j \\\\\n",
    "    &= \\dfrac{n(n+1)}{2} - \\dfrac{\\left[ \\left( \\boxed{k-1} - 1 \\right) + 1 \\right] \\left( \\boxed{k-1}+1 \\right)}{2} \\\\ \n",
    "    &= \\dfrac{n(n+1)}{2} - \\dfrac{(k-1)k}{2} \\\\ \n",
    "    &= \\dfrac{n^2 + n - (k^2 - k)}{2} \\\\\n",
    "    &= \\dfrac{n^2 + n - k^2 + k}{2} \\\\\n",
    "\\end{align}\n",
    "$$\n",
    "\n",
    "Hence\n",
    "\n",
    "$$\n",
    "\\boxed{\\sum_{j=k}^n j = \\dfrac{n^2 + n - k^2 + k}{2}}\n",
    "$$\n",
    "\n",
    "## Step 2: Substitute into Double Sum\n",
    "\n",
    "So we have this\n",
    "\n",
    "$$\n",
    "\\sum_{k=1}^n k^3 = \\sum_{k=1}^n (2k - 1) \\left( \\frac{n^2 + n - k^2 + k}{2} \\right)\n",
    "$$\n",
    "\n",
    "Move the constant out\n",
    "\n",
    "$$\n",
    "\\sum_{k=1}^n k^3 = \\frac{1}{2}\\sum_{k=1}^n (2k - 1) (n^2 + n - k^2 + k)\n",
    "$$\n",
    "\n",
    "$$\n",
    "2\\sum_{k=1}^n k^3 = \\sum_{k=1}^n (2k - 1) (n^2 + n - k^2 + k)\n",
    "$$"
   ]
  },
  {
   "cell_type": "markdown",
   "id": "8862eb02-0290-439e-8767-1e4d04f338d2",
   "metadata": {},
   "source": [
    "## Step 3: Distribute Terms\n",
    "\n",
    "Lets focus on this\n",
    "\n",
    "$$\n",
    "\\textcolor{lightgray}{2\\sum_{k=1}^n k^3 =} \\sum_{k=1}^n (2k - 1)(n^2 + n - k^2 + k)\n",
    "$$\n",
    "\n",
    "Let's expand $(2k - 1)(n^{2}+n - k^{2}+k)$\n",
    "- focus on grouping `k` because the summation is in terms of `k`\n",
    "\n",
    "$$\n",
    "\\begin{align*}\n",
    "    (2k - 1)(n^{2}+n - k^{2}+k) &=2k(n^{2}+n - k^{2}+k)-(n^{2}+n - k^{2}+k)\\\\\n",
    "    &=(2kn^{2}+2kn-2k^{3}+2k^{2})-(n^{2}+n - k^{2}+k)\\\\\n",
    "    &=2kn^{2}+2kn-2k^{3}+2k^{2}-n^{2}-n + k^{2}-k\\\\\n",
    "    &=-2k^{3}+(2k^{2}+k^{2})+2kn+(2kn - k)+( - n^{2}-n)\\\\\n",
    "    &=-2k^{3}+3k^{2}+(2n^{2} + 2n - 1)k - n^{2}-n\n",
    "\\end{align*}\n",
    "$$\n",
    "\n",
    "Thus\n",
    "\n",
    "$$\n",
    "\\textcolor{lightgray}{2\\sum_{k=1}^n k^3 =} \\sum_{k=1}^n \\left[ -2k^{3} + 3k^{2} + (2n^{2} + 2n - 1)k - n^{2} - n \\right]\n",
    "$$\n",
    "\n",
    "Expand\n",
    "$$\n",
    "\\begin{align*}\n",
    "    2\\sum_{k = 1}^{n}k^{3}&=-2\\sum_{k = 1}^{n}k^{3}+3\\sum_{k = 1}^{n}k^{2}+(2n^{2} + 2n - 1)\\sum_{k = 1}^{n}k-\\sum_{k = 1}^{n}n^{2}-\\sum_{k = 1}^{n}n\n",
    "\\end{align*}\n",
    "$$\n",
    "\n",
    "Simplify\n",
    "\n",
    "$$\n",
    "\\begin{align*}\n",
    "    2\\sum_{k = 1}^{n}k^{3}&=-2\\sum_{k = 1}^{n}k^{3}+3 \\cdot \\frac{n(n + 1)(2n + 1)}{6}+(2n^{2} + 2n - 1) \\cdot \\frac{n(n + 1)}{2}-n^{3}-n^{2}\\\\\n",
    "    2\\sum_{k = 1}^{n}k^{3}+2\\sum_{k = 1}^{n}k^{3}&=\\frac{n(n + 1)(2n + 1)}{2}+\\frac{(2n^{2} + 2n - 1)n(n + 1)}{2}-n^{3}-n^{2}\\\\\n",
    "\\end{align*}\n",
    "$$\n",
    "\n",
    "$$\n",
    "\\begin{align*}\n",
    "    4\\sum_{k = 1}^{n}k^{3}&=\\frac{n(n + 1)(2n + 1)+n(n + 1)(2n^{2} + 2n - 1)}{2}-n^{3}-n^{2}\\\\\n",
    "    &=\\frac{n(n + 1)[(2n + 1)+(2n^{2} + 2n - 1)]}{2}-n^{3}-n^{2}\\\\\n",
    "    &=\\frac{n(n + 1)(2n^{2}+4n)}{2}-n^{3}-n^{2}\\\\\n",
    "    &=n(n + 1)(n^{2}+2n)-n^{3}-n^{2}\\\\\n",
    "    &=n(n + 1)(n^{2}+2n)-n(n+1)(n)\\\\\n",
    "    &=n(n + 1)(n^{2}+n)\\\\\n",
    "    &=n(n + 1)[n(n+1)]\\\\\n",
    "    &=n^2 (n+1)^2\n",
    "\\end{align*}\n",
    "$$\n",
    "\n",
    "$$\n",
    "\\begin{align*}\n",
    "    \\sum_{k = 1}^{n}k^{3} &=\\frac{n^2 (n+1)^2}{4} \\\\\n",
    "    &=\\frac{n^2 (n+1)^2}{2^{2}} \\\\\n",
    "    &=\\left[ \\frac{n(n + 1)}{2} \\right] ^{2}\n",
    "\\end{align*}\n",
    "$$\n",
    "\n",
    "---\n",
    "\n",
    "## Conclusion\n",
    "\n",
    "Thus, we have arrived at\n",
    "\n",
    "$$\n",
    "\\boxed{\n",
    "    \\sum_{k = 1}^{n}k^{3} = \\left[ \\frac{n(n + 1)}{2} \\right] ^{2}\n",
    "}\n",
    "$$"
   ]
  }
 ],
 "metadata": {
  "kernelspec": {
   "display_name": "Python 3 (ipykernel)",
   "language": "python",
   "name": "python3"
  },
  "language_info": {
   "codemirror_mode": {
    "name": "ipython",
    "version": 3
   },
   "file_extension": ".py",
   "mimetype": "text/x-python",
   "name": "python",
   "nbconvert_exporter": "python",
   "pygments_lexer": "ipython3",
   "version": "3.12.9"
  }
 },
 "nbformat": 4,
 "nbformat_minor": 5
}
