{
 "cells": [
  {
   "cell_type": "markdown",
   "id": "2f4ed694-3828-4203-a90f-7161e1459a21",
   "metadata": {},
   "source": [
    "# Combinatorial Derivation of Sum of Cubes via Vertical Grouping\n",
    "\n",
    "## Initial Setup\n",
    "We start with the sum of cubes:\n",
    "$$\n",
    "\\sum_{k=1}^n k^3 = 1^3 + 2^3 + \\cdots + n^3\n",
    "$$\n",
    "\n",
    "## Step 1: Expand Cubes as Repeated Addition\n",
    "Each cube term can be expanded vertically:\n",
    "$$\n",
    "\\begin{align*}\n",
    "1^3 &= 1 \\\\\n",
    "2^3 &= (2 + 2) + (2 + 2) \\\\\n",
    "3^3 &= (3 + 3 + 3) + (3 + 3 + 3) + (3 + 3 + 3) \\\\\n",
    "&\\vdots \\\\\n",
    "n^3 &= \\underbrace{\\underbrace{(n + \\cdots + n)}_{n \\text{ times}} + \\cdots + {(n + \\cdots + n)}}_{n \\text{ times}}\n",
    "\\end{align*}\n",
    "$$\n",
    "\n",
    "Notice for the first row, we have $1$ of $1$\n",
    "- for the 2nd row, we have $2^2$ of $2$\n",
    "- for the 3rd row, we have $3^2$ of $3$\n",
    "- ...\n",
    "- This will continue for $n$ rows\n",
    "- for the nth row, we have $n^2$ of $n$\n",
    "\n",
    "This makes sense because\n",
    "\n",
    "$$\n",
    "\\begin{align}\n",
    "    n^3 &= n^2 \\cdot n \\\\\n",
    "    &= n \\cdot n^2 \\\\\n",
    "    &= n \\text{ of } n^2 \\\\\n",
    "\\end{align}\n",
    "$$\n",
    "\n",
    "Hence\n",
    "\n",
    "$$\n",
    "\\text{Number of } n^2 \\text{ is } \\boxed{n}\n",
    "$$\n"
   ]
  },
  {
   "cell_type": "markdown",
   "id": "437e14c6-59cd-44cb-94fa-4da73cd8ce32",
   "metadata": {},
   "source": [
    "## Step 2: Observe Grouping Pattern\n",
    "\n",
    "List out the individual terms that add up to each term in the series\n",
    "\n",
    "$$\n",
    "\\begin{array}{c|ccccccccccc}\n",
    "    1^3 & 1 \\\\\n",
    "    2^3 & 2 & 2 & 2 & 2 \\\\\n",
    "    3^3 & 3 & 3 & 3 & 3 & 3 & 3 & 3 & 3 & 3 \\\\\n",
    "    \\vdots & \\vdots & \\vdots & \\vdots & \\vdots & \\vdots & \\vdots & \\vdots & \\vdots & \\vdots & \\ddots\\\\\n",
    "    n^3 & n & n & n & n & n & n & n & n & n & \\cdots & n\\\\\n",
    "\\end{array}\n",
    "$$\n",
    "\n",
    "By grouping vertically we have\n",
    "\n",
    "$$\n",
    "\\begin{array}{c|c:c:c:c:c:c:c:c:c:cc}\n",
    "    1^3 & 1 \\\\\n",
    "    2^3 & 2 & 2 & 2 & 2 \\\\\n",
    "    3^3 & 3 & 3 & 3 & 3 & 3 & 3 & 3 & 3 & 3 \\\\\n",
    "    \\vdots & \\vdots & \\vdots & \\vdots & \\vdots & \\vdots & \\vdots & \\vdots & \\vdots & \\vdots & \\ddots\\\\\n",
    "    n^3 & n & n & n & n & n & n & n & n & n & \\cdots & n\\\\\n",
    "\\end{array}\n",
    "$$\n",
    "\n",
    "Separate the groups by starting term\n",
    "\n",
    "$$\n",
    "\\begin{array}{c|c:ccc:ccccc:cc}\n",
    "    1^3 & 1 \\\\\n",
    "    2^3 & 2 & 2 & 2 & 2 \\\\\n",
    "    3^3 & 3 & 3 & 3 & 3 & 3 & 3 & 3 & 3 & 3 \\\\\n",
    "    \\vdots & \\vdots & \\vdots & \\vdots & \\vdots & \\vdots & \\vdots & \\vdots & \\vdots & \\vdots & \\ddots\\\\\n",
    "    n^3 & n & n & n & n & n & n & n & n & n & \\cdots & n\\\\\n",
    "\\end{array}\n",
    "$$\n",
    "\n",
    "And we have:\n",
    "\n",
    "$$\n",
    "\\begin{align*}\n",
    "    \\sum_{k=1}^n k^3 &= 1 \\cdot (1 + 2 + \\cdots + n) \\\\\n",
    "    &+ 3 \\cdot (2 + \\cdots + n) \\\\\n",
    "    &+ 5 \\cdot (3 + \\cdots + n) \\\\\n",
    "    &\\vdots \\\\\n",
    "    &+ \\,(2k-1) \\cdot (n) \\,?\\\\\n",
    "\\end{align*}\n",
    "$$\n",
    "\n",
    "It seems that this sum has odd weighted multipliers `e.g. 1, 3, 5`\n",
    "\n",
    "But let's verify it\n"
   ]
  },
  {
   "cell_type": "markdown",
   "id": "c9f99d8b-ece7-473f-9c91-bb37dc419122",
   "metadata": {},
   "source": [
    "## Step 3: Verify the pattern\n",
    "We know that the number of each sequence starting from some number `k` is\n",
    "\n",
    "$$\n",
    "\\begin{align*}\n",
    "    &\\boxed{\\text{Number of raw current sequence: that starts from }k \\text{ of the k-th term}} - \\boxed{\\text{That of the previous sequence: } k-1} \\\\\n",
    "    &= \\boxed{k^2 \\textcolor{gray}{\\text{ of } k}} - \\boxed{(k-1)^2 \\textcolor{gray}{\\text{ of } (k-1)}} \\\\\n",
    "    &= k^2 - (k-1)^2\n",
    "\\end{align*}\n",
    "$$\n",
    "\n",
    "Let's expand and simplify that\n",
    "\n",
    "$$\n",
    "\\begin{align*}\n",
    "    &  k^2 - (k-1)^2 \\\\\n",
    "    &= k^2 - (k^2 - 2k + 1) \\\\\n",
    "    &= \\cancel{k^2} - \\cancel{k^2} + 2k - 1 \\\\\n",
    "    &= 2k - 1\n",
    "\\end{align*}\n",
    "$$\n",
    "\n",
    "Wow! So the difference of squares is also the odd number at that point!\n",
    "\n",
    "$$\n",
    "\\boxed{\n",
    "    \\begin{align*}\n",
    "    &\\text{Difference of squares} \\\\\n",
    "    &= \\text{Odd number} \n",
    "\\end{align*}\n",
    "}\n",
    "$$\n",
    "\n",
    "Thus we can affirm that\n",
    "\n",
    "$$\n",
    "\\begin{align*}\n",
    "    \\sum_{k=1}^n k^3 &= 1 \\cdot (1 + 2 + 3 + \\cdots + n) \\\\\n",
    "    &+ 3 \\cdot (2 + 3 +\\cdots + n)\\\\\n",
    "    &+ 5 \\cdot (3 + \\cdots + n) \\\\\n",
    "    &\\vdots \\\\\n",
    "    &+ (2k - 1)(n) \\\\\n",
    "\\end{align*}\n",
    "$$\n",
    "\n",
    "Thus in summation terms:\n",
    "\n",
    "$$\n",
    "\\begin{align*}\n",
    "    \\sum_{k=1}^n k^3 &= 1 \\cdot \\sum_{j=1}^n j + 3 \\cdot \\sum_{j=2}^n j + 5 \\cdot \\sum_{j=3}^n j + \\cdots + (2k - 1) \\sum_{j=k}^n j \\\\\n",
    "    &= \\underbrace{(2k - 1) \\sum_{j=k}^n j + (2k - 1) \\sum_{j=k}^n j + (2k - 1) \\sum_{j=k}^n j + \\cdots + (2k - 1) \\sum_{j=k}^n j}_{\\text{k from 1 to n}} \\\\\n",
    "    &= \\sum_{k=1}^n \\left[ (2k - 1) \\sum_{j=k}^n j \\right]\n",
    "\\end{align*}\n",
    "$$\n",
    "\n",
    "## Conclusion\n",
    "$$\n",
    "\\boxed{\n",
    "    \\sum_{k=1}^n k^3 = \\sum_{k=1}^n \\left[ (2k - 1) \\sum_{j=k}^n j \\right]\n",
    "}\n",
    "$$"
   ]
  },
  {
   "cell_type": "markdown",
   "id": "fd363c20-2e74-47bb-a5e0-e3e75945e4de",
   "metadata": {},
   "source": [
    "# Derivation of Sum of Cubes from Double-Sum Identity\n",
    "\n",
    "## Given Identity\n",
    "$$\n",
    "\\sum_{k=1}^n k^3 = \\sum_{k=1}^n \\left[ (2k - 1) \\sum_{j=k}^n j \\right]\n",
    "$$\n",
    "\n",
    "## Step 1: Simplify Inner Sum\n",
    "Look at the inner sum\n",
    "\n",
    "$$\n",
    "\\textcolor{lightgray}{\\sum_{k=1}^n k^3 = \\sum_{k=1}^n} \\left[ \\textcolor{lightgray}{(2k - 1)} \\sum_{j=k}^n j \\right]\n",
    "$$\n",
    "\n",
    "We can derive the general form of the sum of squares by removing a part from the whole\n",
    "\n",
    "$$\n",
    "\\begin{align}\n",
    "    \\sum_{j=k}^n j &= \\sum_{j=1}^n j - \\sum_{j=1}^{k-1} j \\\\\n",
    "    &= \\dfrac{n(n+1)}{2} - \\dfrac{\\left[ \\left( \\boxed{k-1} - 1 \\right) + 1 \\right] \\left( \\boxed{k-1}+1 \\right)}{2} \\\\ \n",
    "    &= \\dfrac{n(n+1)}{2} - \\dfrac{(k-1)k}{2} \\\\ \n",
    "    &= \\dfrac{n^2 + n - (k^2 - k)}{2} \\\\\n",
    "    &= \\dfrac{n^2 + n - k^2 + k}{2} \\\\\n",
    "\\end{align}\n",
    "$$\n",
    "\n",
    "Hence\n",
    "\n",
    "$$\n",
    "\\boxed{\\sum_{j=k}^n j = \\dfrac{n^2 + n - k^2 + k}{2}}\n",
    "$$\n",
    "\n",
    "## Step 2: Substitute into Double Sum\n",
    "\n",
    "So we have this\n",
    "\n",
    "$$\n",
    "\\sum_{k=1}^n k^3 = \\sum_{k=1}^n (2k - 1) \\left( \\frac{n^2 + n - k^2 + k}{2} \\right)\n",
    "$$\n",
    "\n",
    "Move the constant out\n",
    "\n",
    "$$\n",
    "\\sum_{k=1}^n k^3 = \\frac{1}{2}\\sum_{k=1}^n (2k - 1) (n^2 + n - k^2 + k)\n",
    "$$\n",
    "\n",
    "$$\n",
    "2\\sum_{k=1}^n k^3 = \\sum_{k=1}^n (2k - 1) (n^2 + n - k^2 + k)\n",
    "$$"
   ]
  },
  {
   "cell_type": "markdown",
   "id": "41e282f5-3fd2-4bc2-8878-7e98778b18cc",
   "metadata": {},
   "source": [
    "## Step 3: Distribute Terms\n",
    "\n",
    "Lets focus on this\n",
    "\n",
    "$$\n",
    "\\textcolor{lightgray}{2\\sum_{k=1}^n k^3 =} \\sum_{k=1}^n (2k - 1)(n^2 + n - k^2 + k)\n",
    "$$\n",
    "\n",
    "Notice that $\\boxed{n^2 + n}$ is unaffected by the summation, thus a constant. \n",
    "\n",
    "We can find a way to factor it out\n",
    "\n",
    "$$\n",
    "\\sum_{k=1}^n (2k - 1)\\left[ (n^2 + n) - (k^2 - k) \\right]\n",
    "$$\n",
    "\n",
    "$$\n",
    "\\sum_{k=1}^n \\boxed{(2k - 1)(n^2 + n) - (2k - 1)(k^2 - k)}\n",
    "$$\n",
    "\n",
    "$$\n",
    "\\sum_{k=1}^n (2k - 1)(n^2 + n) - \\sum_{k=1}^n (2k - 1)(k^2 - k)\n",
    "$$\n",
    "\n",
    "$$\n",
    "(n^2 + n)\\sum_{k=1}^n (2k - 1) - \\sum_{k=1}^n (2k - 1)(k^2 - k)\n",
    "$$\n",
    "\n",
    "Thus\n",
    "\n",
    "$$\n",
    "2\\sum_{k=1}^n k^3 = (n^2 + n)\\sum_{k=1}^n (2k - 1) - \\sum_{k=1}^n (2k - 1)(k^2 - k)\n",
    "$$\n",
    "\n",
    "We can focus on each part separately"
   ]
  },
  {
   "cell_type": "markdown",
   "id": "74424c1b-e336-4a9c-aa67-3aeb9f8b9f16",
   "metadata": {},
   "source": [
    "## Part 1: Sum of Odds\n",
    "\n",
    "Lets look at this\n",
    "\n",
    "$$\n",
    "\\textcolor{lightgray}{2\\sum_{k=1}^n k^3 =} (n^2 + n)\\sum_{k=1}^n (2k - 1) \\textcolor{lightgray}{- \\sum_{k=1}^n (2k - 1)(k^2 - k)}\n",
    "$$\n",
    "\n",
    "Even more specifically at this\n",
    "$$\n",
    "\\textcolor{lightgray}{(n^2 + n)} \\sum_{k=1}^n (2k - 1)\n",
    "$$\n",
    "\n",
    "---\n",
    "\n",
    "This is a known cool identity\n",
    "\n",
    "$$\n",
    "\\boxed{\\sum_{k=1}^n (2k - 1) = n^2}\n",
    "$$\n",
    "\n",
    "But let's prove it since its simple and quick\n",
    "\n",
    "$$\n",
    "\\begin{align*}\n",
    "    \\sum_{k=1}^n (2k - 1) &= 2\\sum_{k=1}^n k - \\sum_{k=1}^n 1 \\\\\n",
    "    &= \\cancel{2} \\cdot \\dfrac{n(n+1)}{\\cancel{2}} - n \\\\\n",
    "    &= (n^2 + \\cancel{n}) - \\cancel{n} \\\\\n",
    "    &= n^2\n",
    "\\end{align*}\n",
    "$$\n",
    "\n",
    "---\n",
    "\n",
    "And use it here\n",
    "$$\n",
    "\\begin{align*}\n",
    "    (n^2 + n) \\sum_{k=1}^n (2k - 1) &= (n^2 + n) \\cdot n^2 \\\\\n",
    "    &= n^4+n^3 \n",
    "\\end{align*}\n",
    "$$\n",
    "\n",
    "Thus\n",
    "\n",
    "$$\n",
    "2\\sum_{k=1}^n k^3 = n^4 + n^3 - \\sum_{k=1}^n (2k - 1)(k^2 - k)\n",
    "$$"
   ]
  },
  {
   "cell_type": "markdown",
   "id": "d27c1b2e-d2e4-4b86-a8c8-b67515c86ca3",
   "metadata": {},
   "source": [
    "## Part 2: Polynomial Expansion\n",
    "\n",
    "Now lets look at this\n",
    "\n",
    "$$\n",
    "\\textcolor{lightgray}{2\\sum_{k=1}^n k^3 = n^4 + n^3} \\textcolor{lightgray}{-} \\sum_{k=1}^n (2k - 1)(k^2 - k)\n",
    "$$\n",
    "\n",
    "Zoom in to this\n",
    "$$\n",
    "\\textcolor{lightgray}{\\sum_{k=1}^n} (2k - 1)(k^2 - k)\n",
    "$$\n",
    "\n",
    "Lets expand and simplify\n",
    "\n",
    "$$\n",
    "\\begin{align*}\n",
    "    (2k - 1)(k^2 - k) &= 2k^3 - 2k^2 - k^2 + k \\\\\n",
    "    &= 2k^3 - 3k^2 + k\n",
    "\\end{align*}\n",
    "$$\n",
    "\n",
    "Substitute back\n",
    "$$\n",
    "\\sum_{k=1}^n (2k^3 - 3k^2 + k)\n",
    "$$\n",
    "\n",
    "Expand and simplify\n",
    "$$\n",
    "\\begin{align*}\n",
    "    \\sum_{k=1}^n (2k^3 - 3k^2 + k) &= 2\\sum_{k=1}^n k^3 - 3\\sum_{k=1}^n k^2 + \\sum_{k=1}^n k \\\\\n",
    "    &= 2\\sum_{k=1}^n k^3 - \\cancel{3}\\left[ \\frac{n(n+1)(2n+1)}{\\cancel{6} 2} \\right] + \\frac{n(n+1)}{2} \\\\\n",
    "    &= 2\\sum_{k=1}^n k^3 - \\left[ \\frac{n(n+1)(2n+1)}{2} \\right] + \\frac{n(n+1)}{2}\n",
    "\\end{align*}\n",
    "$$\n",
    "\n",
    "Thus\n",
    "\n",
    "$$\n",
    "2\\sum_{k=1}^n k^3  = n^4 + n^3 - \\left[ 2\\sum_{k=1}^n k^3 - \\left( \\frac{n(n+1)(2n+1)}{2} \\right) + \\frac{n(n+1)}{2} \\right]\n",
    "$$"
   ]
  },
  {
   "cell_type": "markdown",
   "id": "2c5a7445-33d5-4fe9-a543-20cb74a53e98",
   "metadata": {
    "jp-MarkdownHeadingCollapsed": true
   },
   "source": [
    "## Step 4: Combine Results\n",
    "\n",
    "$$\n",
    "\\begin{align*}\n",
    "    2\\sum_{k=1}^n k^3 &= n^4 + n^3 - \\left[ 2\\sum_{k=1}^n k^3 - \\left( \\frac{n(n+1)(2n+1)}{2} \\right) + \\frac{n(n+1)}{2} \\right] \\\\\n",
    "    &= n^4 + n^3 - 2\\sum_{k=1}^n k^3 + \\left( \\frac{n(n+1)(2n+1)}{2} \\right) - \\frac{n(n+1)}{2} \\\\\n",
    "\\end{align*}\n",
    "$$\n",
    "\n",
    "$$\n",
    "4\\sum_{k=1}^n k^3 = n^4 + n^3 + \\left( \\frac{n(n+1)(2n+1)}{2} \\right) - \\frac{n(n+1)}{2}\n",
    "$$\n",
    "\n",
    "$$\n",
    "4\\sum_{k=1}^n k^3 = n^2 \\cdot n(n+1) + \\left( \\frac{n(n+1)(2n+1)}{2} \\right) - \\frac{n(n+1)}{2}\n",
    "$$\n",
    "\n",
    "$$\n",
    "\\begin{align*}\n",
    "    8\\sum_{k=1}^n k^3 &= 2n^2 \\cdot n(n+1) + (2n+1)[n(n+1)] - n(n+1) \\\\\n",
    "    &= [2n^2 + (2n + 1) - 1][n(n+1)] \\\\\n",
    "    &= [2n^2 + 2n][n(n+1)]\n",
    "\\end{align*}\n",
    "$$\n",
    "\n",
    "$$\n",
    "4\\sum_{k=1}^n k^3 = [n^2 + n][n(n+1)]\n",
    "$$\n",
    "\n",
    "$$\n",
    "4\\sum_{k=1}^n k^3 = [n(n+1)][n(n+1)]\n",
    "$$\n",
    "\n",
    "$$\n",
    "\\begin{align*}\n",
    "    \\sum_{k=1}^n k^3 &= \\dfrac{[n(n+1)]^2}{4} \\\\\n",
    "    &= \\dfrac{[n(n+1)]^2}{2^2} \\\\\n",
    "    &= \\left[ \\dfrac{n(n+1)}{2} \\right]^2\n",
    "\\end{align*}\n",
    "$$\n",
    "\n",
    "---\n",
    "\n",
    "## Conclusion\n",
    "\n",
    "Therefore, we have proven\n",
    "\n",
    "$$\n",
    "\\boxed{\n",
    "    \\sum_{k=1}^n k^3 = \\left[ \\dfrac{n(n+1)}{2} \\right]^2\n",
    "}\n",
    "$$"
   ]
  }
 ],
 "metadata": {
  "kernelspec": {
   "display_name": "Python 3 (ipykernel)",
   "language": "python",
   "name": "python3"
  },
  "language_info": {
   "codemirror_mode": {
    "name": "ipython",
    "version": 3
   },
   "file_extension": ".py",
   "mimetype": "text/x-python",
   "name": "python",
   "nbconvert_exporter": "python",
   "pygments_lexer": "ipython3",
   "version": "3.12.9"
  }
 },
 "nbformat": 4,
 "nbformat_minor": 5
}
