{
 "cells": [
  {
   "cell_type": "markdown",
   "id": "bf181a97-9cfe-43ae-b76f-793225908869",
   "metadata": {},
   "source": [
    "# Combinatorial Approach to the Sum of Squares Formula\n",
    "\n",
    "We derive the formula for the sum of squares using a combinatorial approach by expressing the sum as a double summation, applying the arithmetic sequence formula, and then using algebraic manipulation.\n",
    "\n",
    "---\n",
    "Before Anything lets play with the sum a little\n",
    "\n",
    "# Algebraic Manipulation\n",
    "Let's seek to make the exponential into an addition problem\n",
    "$$\n",
    "\\sum_{k=1}^n k^2 = 1^2 + 2^2 + 3^2 + ... + n^2\n",
    "$$\n",
    "\n",
    "$$\n",
    "\\sum_{k=1}^n k^2 = (1 \\cdot 1) + (2 \\cdot 2) + (3 \\cdot 3) + ... + (n \\cdot n)\n",
    "$$\n",
    "\n",
    "$$\n",
    "\\sum_{k=1}^n k^2 = 1 + (2 + 2) + (3 + 3 + 3) + ... + (\\underbrace{n + n + \\dots + n}_{n \\text{ times}})\n",
    "$$\n",
    "\n",
    "Arrange it vertically so that each term's contribution is clear\n",
    "\n",
    "$$\n",
    "\\begin{align*}\n",
    "    \\sum_{k=1}^n k^2 &= 1 \\\\\n",
    "    &\\quad + (2 + 2) \\\\\n",
    "    &\\quad + (3 + 3 + 3) \\\\\n",
    "    &\\quad \\vdots \\\\ \n",
    "    &\\quad + (\\underbrace{n + n + \\dots + n}_{n \\text{ times}})\n",
    "\\end{align*}\n",
    "$$\n",
    "\n",
    "By grouping vertically (or taking the nth term of every group) we have:\n",
    "\n",
    "$$\n",
    "\\sum_{k=1}^n k^2 = \\underbrace{(1 + 2 + 3 + ... + n) + (2 + 3 + 4 + ... + n) + ... + n}_{n \\text{ terms}}\n",
    "$$\n",
    "\n",
    "Let's describe every individual summation with a new index `j`\n",
    "\n",
    "$$\n",
    "\\sum_{k=1}^n k^2 = \\underbrace{\\sum_{j=1}^n j + \\sum_{j=2}^n j + ... + \\sum_{j=n}^n j}_{n \\text{ terms}}\n",
    "$$\n",
    "\n",
    "Observe that the starting index of every individual sum, `j`, follows from its current term index, which can be described by another variable.\n",
    "For which we can reuse the variable `k`, to count the progression of `j` from `1` to `n`\n",
    "$$\n",
    "\\sum_{k=1}^n \\sum_{j=k}^{n} j\n",
    "$$\n",
    "\n",
    "Therefore, we have gotten this identity described in a Double Summation:\n",
    "$$\n",
    "\\boxed{\\sum_{k=1}^n k^2 = \\sum_{k=1}^n \\sum_{j=k}^{n} j}\n",
    "$$"
   ]
  },
  {
   "attachments": {},
   "cell_type": "markdown",
   "id": "fe7e0630-ade2-4eed-b0f9-c9fc218cd7ef",
   "metadata": {},
   "source": [
    "# Visualising the Sum in 2 Dimensions\n",
    "Sometimes, it's not convincing enough to do it algebraically\n",
    "\n",
    "So let's visualise this transformation in a table\n",
    "\n",
    "$$\n",
    "\\sum_{k=1}^n k^2 = 1^2 + 2^2 + 3^2 + ... + n^2\n",
    "$$\n",
    "\n",
    "can be visualised like this:\n",
    "\n",
    "$$\n",
    "\\begin{array}{c|ccccccc}\n",
    "    k=1 & 1 \\\\\n",
    "    k=2 & 2 & 2 \\\\\n",
    "    k=3 & 3 & 3 & 3 \\\\\n",
    "    k=4 & 4 & 4 & 4 & 4 \\\\\n",
    "    k=5 & 5 & 5 & 5 & 5 & 5 \\\\\n",
    "    \\vdots & \\vdots & \\vdots & \\vdots & \\vdots & \\vdots & \\ddots \\\\\n",
    "    k=n & n & n & n & n & n & \\cdots & n \\\\\n",
    "\\end{array}\n",
    "$$\n",
    "\n",
    "Notice that the horizontal index also goes from 1 to n:\n",
    "\n",
    "$$\n",
    "\\begin{array}{c|ccccc}\n",
    "    & j=1 & j=2 & j=3 & \\cdots & \\cdots & \\cdots & j=n \\\\\n",
    "\\hline\n",
    "    k=1 & 1 \\\\\n",
    "    k=2 & 2 & 2 \\\\\n",
    "    k=3 & 3 & 3 & 3 \\\\\n",
    "    k=4 & 4 & 4 & 4 & 4 \\\\\n",
    "    k=5 & 5 & 5 & 5 & 5 & 5 \\\\\n",
    "    \\vdots & \\vdots & \\vdots & \\vdots & \\vdots & \\vdots & \\ddots \\\\\n",
    "    k=n & n & n & n & n & n & \\cdots & n \\\\\n",
    "\\end{array}\n",
    "$$\n",
    "\n",
    "Notice that vertical sums gives arithmetic sums\n",
    "\n",
    "$$\n",
    "\\begin{array}{c|ccccc}\n",
    "    & j=1 & j=2 & j=3 & \\cdots & \\cdots & \\cdots & j=n \\\\\n",
    "\\hline\n",
    "    k=1 & 1 \\\\\n",
    "    k=2 & 2 & 2 \\\\\n",
    "    k=3 & 3 & 3 & 3 \\\\\n",
    "    k=4 & 4 & 4 & 4 & 4 \\\\\n",
    "    k=5 & 5 & 5 & 5 & 5 & 5 \\\\\n",
    "    \\vdots & \\vdots & \\vdots & \\vdots & \\vdots & \\vdots & \\ddots \\\\\n",
    "    k=n & n & n & n & n & n & \\cdots & n \\\\\n",
    "\\hline\n",
    "    & \\sum_{j=1}^{n} j & \\sum_{j=2}^{n} j & \\sum_{j=3}^{n} j & \\sum_{j=4}^{n} j & \\sum_{j=5}^{n} j & \\cdots & \\sum_{j=n}^{n} j\n",
    "\\end{array}\n",
    "$$\n",
    "\n",
    "Okay great, now we can sum up all the sums of `j` to `n` for every `j` from `1` to `n`\n",
    "\n",
    "$$\n",
    "\\sum_{k=1}^n k^2 = \\underbrace{\\sum_{j=1}^n j + \\sum_{j=2}^n j + ... + \\sum_{j=n}^n j}_{n \\text{ terms}}\n",
    "$$\n",
    "\n",
    "We cannot use the same variable `j` for the change in starting value for each sum, because it already describes each individual arithmetic sum\n",
    "\n",
    "So we gotta pick another variable!\n",
    "\n",
    "Notice that `k` also progresses from `1` to `n`, equalling the progression of the starting value `j`\n",
    "\n",
    "$$\n",
    "\\begin{array}{c|ccccc}\n",
    "    & j=1 & j=2 & j=3 & \\cdots & \\cdots & \\cdots & j=n \\\\\n",
    "\\hline\n",
    "    k=1 & 1 \\\\\n",
    "    k=2 & 2 & 2 \\\\\n",
    "    k=3 & 3 & 3 & 3 \\\\\n",
    "    k=4 & 4 & 4 & 4 & 4 \\\\\n",
    "    k=5 & 5 & 5 & 5 & 5 & 5 \\\\\n",
    "    \\vdots & \\vdots & \\vdots & \\vdots & \\vdots & \\vdots & \\ddots \\\\\n",
    "    k=n & n & n & n & n & n & \\cdots & n \\\\\n",
    "\\hline\n",
    "    & \\sum_{j=k}^{n} j & \\sum_{j=k}^{n} j & \\sum_{j=k}^{n} j & \\sum_{j=k}^{n} j & \\sum_{j=k}^{n} j & \\cdots & \\sum_{j=k}^{n} j\n",
    "\\end{array}\n",
    "$$\n",
    "\n",
    "Therefore, we can let `j` be described in terms of `k`, \n",
    "\n",
    "as in `j = k`, for `k` from `1` to `n`\n",
    "\n",
    "$$\n",
    "\\sum_{k=1}^n k^2 = \\underbrace{\\sum_{j=k}^{n} j + \\sum_{j=k}^{n} j + ... + \\sum_{j=k}^{n} j}_{\\text{For k from 1 to n}}\n",
    "$$\n",
    "\n",
    "Re-write that in mathematical notation, and we have:\n",
    "\n",
    "$$\n",
    "\\boxed{\\sum_{k=1}^n k^2 = \\sum_{k=1}^n \\sum_{j=k}^{n} j}\n",
    "$$"
   ]
  },
  {
   "cell_type": "markdown",
   "id": "7497034d-9c6f-4bb2-9dda-43ebe8bdfb1e",
   "metadata": {},
   "source": [
    "# Apply the Arithmetic Sequence Formula\n",
    "\n",
    "Now we know with justification that \n",
    "$$ \n",
    "\\sum_{k=1}^n k^2 = \\sum_{k=1}^n \\sum_{j=k}^{n} j \n",
    "$$\n",
    "\n",
    "Let's focus on the inner sum \n",
    "\n",
    "$$ \n",
    "\\quad \\sum_{j=k}^n j \\quad \n",
    "$$ \n",
    "\n",
    "Notice it is an arithmetic sequence with:\n",
    "\n",
    "- First term = $k$\n",
    "- Last term = $n$\n",
    "- Common Difference = $d$ = $1$\n",
    "\n",
    "- $\n",
    "\\begin{aligned}\n",
    "    \\text{Number of terms} &= \\frac{n - k}{d}+1 \\space \\text{ (Difference of Terms + 1)}\\\\\n",
    "    &= \\frac{n - k}{1}+1 \\\\\n",
    "    &= n - k + 1\n",
    "\\end{aligned}\n",
    "$\n",
    "\n",
    "The sum of this arithmetic sequence is therefore:\n",
    "\n",
    "$$\n",
    "\\left( \n",
    "    \\dfrac{\\text{first term} + \\text{last term}}{2} \n",
    "\\right) (\\text{number of terms})\n",
    "$$\n",
    "\n",
    "$$\n",
    "\\left( \n",
    "    \\dfrac{n + k}{2} \n",
    "\\right) (n - k + 1)\n",
    "$$\n",
    "\n",
    "$$\n",
    "\\dfrac{(n + k)(n - k + 1)}{2}\n",
    "$$\n",
    "\n",
    "Thus:\n",
    "\n",
    "$$\n",
    "\\sum_{k=1}^n \\dfrac{(n + k)(n - k + 1)}{2}\n",
    "$$\n",
    "\n",
    "Factor out $\\dfrac{1}{2}$:\n",
    "\n",
    "$$\n",
    "\\dfrac{1}{2} \\sum_{k=1}^n (n + k)(n - k + 1)\n",
    "$$"
   ]
  },
  {
   "cell_type": "markdown",
   "id": "7c7e81de-c151-4a83-b15c-b7aaf5dc4765",
   "metadata": {},
   "source": [
    "# Simplify the Inner Expression\n",
    "\n",
    "Expand the inner expression $(n + k)(n - k + 1)$:\n",
    "\n",
    "$$\n",
    "\\begin{aligned}\n",
    "    (n + k)(n - k + 1) &= n^2 - nk + n + kn - k^2 + k \\\\\n",
    "                       &= n^2 + n - k^2 + k\n",
    "\\end{aligned}\n",
    "$$\n",
    "\n",
    "Substitute back into the sum:\n",
    "\n",
    "$$\n",
    "\\dfrac{1}{2} \\sum_{k=1}^n (n^2 + n - k^2 + k)\n",
    "$$\n",
    "\n",
    "Break into individual sums:\n",
    "\n",
    "$$\n",
    "\\dfrac{1}{2} \\left( \n",
    "    \\sum_{k=1}^n n^2 + \\sum_{k=1}^n n - \\sum_{k=1}^n k^2 + \\sum_{k=1}^n k \n",
    "\\right)\n",
    "$$\n",
    "\n",
    "---\n",
    "\n",
    "Zoom in to the summations:\n",
    "\n",
    "$$\n",
    "\\sum_{k=1}^n n^2 + \\sum_{k=1}^n n - \\sum_{k=1}^n k^2 + \\sum_{k=1}^n k \n",
    "$$\n",
    "\n",
    "Notice that these 2 summations are simplifiable\n",
    "\n",
    "$$\n",
    "\\sum_{k=1}^n n^2 + \\sum_{k=1}^n n \\textcolor{lightgray}{- \\sum_{k=1}^n k^2 + \\sum_{k=1}^n k}\n",
    "$$\n",
    "\n",
    "$$\n",
    "n^3 + n^2 \\textcolor{lightgray}{- \\sum_{k=1}^n k^2 + \\sum_{k=1}^n k}\n",
    "$$\n",
    "\n",
    "Notice that the expansion contains the sum we want to find itself:\n",
    "\n",
    "$$\n",
    "\\textcolor{lightgray}{n^3 + n^2} - \\sum_{k=1}^n k^2 + \\textcolor{lightgray}{\\sum_{k=1}^n k}\n",
    "$$\n",
    "\n",
    "Notice that the last term is describing an arithmetic sequence\n",
    "\n",
    "$$ \n",
    "\\textcolor{lightgray}{n^3 + n^2 - \\sum_{k=1}^n k^2} + \\sum_{k=1}^n k \n",
    "$$\n",
    "\n",
    "$$ \n",
    "\\textcolor{lightgray}{n^3 + n^2 - \\sum_{k=1}^n k^2} + \\dfrac{n(n+1)}{2}\n",
    "$$\n",
    "\n",
    "---\n",
    "\n",
    "Hence, it simplifies to:\n",
    "\n",
    "$$\n",
    "\\dfrac{1}{2} \\left[ \n",
    "    n^3 + n^2 - \\sum_{k=1}^n k^2 + \\dfrac{n(n+1)}{2} \n",
    "\\right]\n",
    "$$\n",
    "\n",
    "Since\n",
    "$$\n",
    "\\sum_{k=1}^n k^2 = \\dfrac{1}{2} \\left[ \n",
    "    n^3 + n^2 - \\sum_{k=1}^n k^2 + \\dfrac{n(n+1)}{2} \n",
    "\\right]\n",
    "$$\n",
    "\n",
    "To make writing easier, let \n",
    "$$\n",
    "\\mathbf{S_n} = \\sum_{k=1}^n k^2\n",
    "$$\n",
    "\n",
    "Hence\n",
    "$$\n",
    "\\mathbf{S_n} = \\dfrac{1}{2} \\left[ \n",
    "    n^3 + n^2 - \\mathbf{S_n} + \\dfrac{n(n+1)}{2} \n",
    "\\right]\n",
    "$$\n",
    "\n",
    "---\n",
    "\n",
    "Balance the equation:\n",
    "\n",
    "$$\n",
    "2\\space\\mathbf{S_n} = n^3 + n^2 - \\mathbf{S_n} + \\dfrac{n(n+1)}{2}\n",
    "$$\n",
    "\n",
    "$$\n",
    "3\\space\\mathbf{S_n} = n^3 + n^2 + \\dfrac{n(n+1)}{2}\n",
    "$$\n",
    "\n",
    "$$\n",
    "3\\space\\mathbf{S_n} = \\dfrac{2n^3 + 2n^2 + n^2 + n}{2}\n",
    "$$\n",
    "\n",
    "$$\n",
    "\\begin{aligned}\n",
    "    \\mathbf{S_n} &= \\dfrac{2n(n^2 + n) + (n^2 + n)}{6} \\\\\n",
    "    \\mathbf{S_n} &= \\dfrac{(n^2 + n)(2n + 1)}{6} \\\\\n",
    "    \\mathbf{S_n} &= \\dfrac{n(n + 1)(2n + 1)}{6}\n",
    "\\end{aligned}\n",
    "$$\n",
    "\n",
    "Therefore:\n",
    "\n",
    "$$\n",
    "\\boxed{ \\sum_{k=1}^n k^2 = \\dfrac{n(n + 1)(2n + 1)}{6} }\n",
    "$$"
   ]
  },
  {
   "cell_type": "markdown",
   "id": "9df98598-40c8-42cb-9391-77e345f80586",
   "metadata": {},
   "source": [
    "# General Sum of Squares\n",
    "\n",
    "The general sum is\n",
    "\n",
    "$$\n",
    "\\sum_{k=j}^n k^2 = \\dfrac{n(n + 1)(2n + 1)}{6}\n",
    "$$\n",
    "\n",
    "Expand by making it a difference of two sums from `1` to `m`\n",
    "\n",
    "$$\n",
    "\\begin{align*}\n",
    "    \\sum_{k=j}^n k^2 &= \\sum_{k=1}^n k^2 - \\sum_{k=1}^{j-1} k^2 \\\\\n",
    "    &= \\dfrac{n(n + 1)(2n + 1)}{6} - \\dfrac{(j-1)[(j-1) + 1][2(j-1) + 1]}{6}\\\\\n",
    "    &= \\dfrac{n(n + 1)(2n + 1)}{6} - \\dfrac{(j-1)j(2j-2 + 1)}{6}\\\\\n",
    "    &= \\dfrac{n(n + 1)(2n + 1)}{6} - \\dfrac{(j-1)j(2j-1)}{6}\\\\\n",
    "    &= \\dfrac{n(n + 1)(2n + 1) - j(j-1)(2j-1)}{6} \\\\\n",
    "    &= \\dfrac{1}{6} \\biggr[ n(n + 1)(2n + 1) - j(j-1)(2j-1) \\biggr] \\\\\n",
    "\\end{align*}\n",
    "$$\n",
    "\n",
    "Thus\n",
    "\n",
    "$$\n",
    "\\boxed{\n",
    "    \\sum_{k=j}^n k^2 =  \\dfrac{1}{6} \\biggr[ n(n + 1)(2n + 1) - j(j-1)(2j-1) \\biggr]\n",
    "}\n",
    "$$"
   ]
  },
  {
   "cell_type": "markdown",
   "id": "74cd952f-7048-45f9-bd47-aac57794db75",
   "metadata": {},
   "source": [
    "# Additional Insights\n",
    "\n",
    "## Initial Analysis\n",
    "\n",
    "From this we can see that also:\n",
    "\n",
    "$$\n",
    "\\textcolor{lightgray}{\\sum_{k=1}^n k^2 = \\left( \\dfrac{2n + 1}{3} \\right)} \\left( \\dfrac{n(n + 1)}{2} \\right)\n",
    "$$\n",
    "\n",
    "$$\n",
    "\\textcolor{lightgray}{\\sum_{k=1}^n k^2 = \\left( \\dfrac{2n + 1}{3} \\right)} \\sum_{k=1}^n k\n",
    "$$\n",
    "\n",
    "$$\n",
    "\\sum_{k=1}^n k^2 = \\left( \\dfrac{2n + 1}{3} \\right) \\sum_{k=1}^n k\n",
    "$$\n",
    "\n",
    "Thus, the sum of squares is the common arithmetic sum by a factor of $ \\boxed{\\frac{2n + 1}{3}} $\n",
    "\n",
    "$$\n",
    "\\boxed{\n",
    "    \\text{Sum of squares} \\space = \\left( \\dfrac{2n + 1}{3} \\right) \\space \\text{of Arithmetic sum}\n",
    "}\n",
    "$$\n",
    "\n",
    "But we can go further!\n",
    "\n",
    "## Average and Total\n",
    "\n",
    "Notice that when the series is expanded:\n",
    "\n",
    "$$\n",
    "\\begin{align*}\n",
    "    \\sum_{k=1}^n k^2 &= 1 \\\\\n",
    "    &\\quad + (2 + 2) \\\\\n",
    "    &\\quad + (3 + 3 + 3) \\\\\n",
    "    &\\quad \\vdots \\\\ \n",
    "    &\\quad + (\\underbrace{n + n + \\dots + n}_{n \\text{ times}})\n",
    "\\end{align*}\n",
    "$$\n",
    "\n",
    "Each row `i.e. nth row` contributes exactly `n` terms `i.e. 1 + 2 + 3 + ... + n`\n",
    "\n",
    "Which means the total number of terms in the addition is equal to the arithmetic sum \n",
    "\n",
    "$$\n",
    "1 + 2 + 3 + ... + n =  \\sum_{k=1}^n k\n",
    "$$\n",
    "\n",
    "Thus\n",
    "\n",
    "$$\n",
    "\\underline{\n",
    "    \\text{Total number of Addition Terms} = \\text{Arithmetic Sum}\n",
    "}\n",
    "$$\n",
    "\n",
    "And since\n",
    "\n",
    "$$\n",
    "\\sum_{k=1}^n k = \\dfrac{n(n + 1)}{2} = \\text{Arithmetic Sum} = \\text{Total number of Addition Terms}\n",
    "$$\n",
    "\n",
    "And\n",
    "\n",
    "$$\n",
    "\\textcolor{lightgray}{\\sum_{k=1}^n k^2 = \\left( \\dfrac{2n + 1}{3} \\right)} \\cdot \\text{Total number of Addition Terms}\n",
    "$$\n",
    "\n",
    "It makes the other part of the formula\n",
    "\n",
    "$$\n",
    "\\textcolor{lightgray}{\\sum_{k=1}^n k^2 =} \\left( \\dfrac{2n + 1}{3} \\right) \\textcolor{lightgray}{\\cdot \\text{Total number of Addition Terms}}\n",
    "$$\n",
    "\n",
    "Equivalent to the average of those addition terms\n",
    "\n",
    "$$\n",
    "\\textcolor{lightgray}{\\sum_{k=1}^n k^2 =} \\text{Average of Addition Terms} \\textcolor{lightgray}{\\cdot \\text{Total number of Addition Terms}}\n",
    "$$\n",
    "\n",
    "Thus\n",
    "\n",
    "$$\n",
    "\\boxed{\n",
    "    \\text{Average of Addition Terms} = \\left( \\dfrac{2n + 1}{3} \\right)\n",
    "}\n",
    "$$\n",
    "\n",
    "And\n",
    "\n",
    "$$\n",
    "\\underline{\n",
    "    \\text{Sum of squares} = \\text{Average of Addition Terms} \\cdot \\text{Total number of Addition Terms}\n",
    "}\n",
    "$$\n",
    "\n",
    "But theres more!\n",
    "\n",
    "## Relationship to the Next Odd Number\n",
    "\n",
    "Notice this\n",
    "\n",
    "$$\n",
    "\\textcolor{lightgray}{\\text{Average of Addition Terms} =} \\textcolor{lightgray}{\\biggr(} \\dfrac{2n + 1}{\\textcolor{lightgray}{3}} \\textcolor{lightgray}{\\biggr)}\n",
    "$$\n",
    "\n",
    "It can represent all the odd numbers if we let `n` start from `0`\n",
    "\n",
    "$$\n",
    "\\text{Odd Numbers} \\space = \\{ 1, 3, 5, 7, \\cdots\\} = \\{2n+1 ∣ n= 0, 1, 2 \\cdots \\}\n",
    "$$\n",
    "\n",
    "But since `n` starts from `1`, `2n+1` represents the odd numbers from `3` onwards\n",
    "\n",
    "$$\n",
    "\\text{Odd Numbers from 3} \\space = \\{ 3, 5, 7, \\cdots\\} = \\{2n+1 ∣ n= 1, 2, 3 \\cdots \\}\n",
    "$$\n",
    "\n",
    "It is always one iteration more on the scale of all odd numbers\n",
    "- Represented by `2n-1`\n",
    "\n",
    "$$\n",
    "\\text{Odd Numbers} \\space = \\{ 1, 3, 5, 7, \\cdots\\} = \\{2n-1 ∣ n= 1, 2, 3 \\cdots \\}\n",
    "$$\n",
    "\n",
    "- The next odd number `i.e. one iteration more`\n",
    "\n",
    "$$\n",
    "\\text{Next Odd Number} \\space = \\{ \\_, 3, 5, 7, \\cdots\\} = \\{2n-1 ∣ n= \\_ , 2, 3 \\cdots \\}\n",
    "$$\n",
    "\n",
    "Thus\n",
    "\n",
    "$$\n",
    "\\boxed{\n",
    "    \\text{Average of Addition Terms} = \\dfrac{\\text{Next Odd Number}}{3}\n",
    "}\n",
    "$$\n"
   ]
  },
  {
   "cell_type": "markdown",
   "id": "4eb2d0e8-1e45-4725-a854-d04afda0b5a4",
   "metadata": {},
   "source": [
    "# Conclusion\n",
    "\n",
    "Therefore, we get\n",
    "\n",
    "$$\n",
    "\\text{Sum of squares} \\space = \\text{Average of Addition Terms} \\cdot \\space \\text{Number of Addition Terms}\n",
    "$$\n",
    "\n",
    "Where\n",
    "\n",
    "$$\n",
    "\\begin{align*}\n",
    "    &\\underline{\\text{Average of Addition Terms}} = \\text{A Third of the Next Odd Number} = \\dfrac{2n + 1}{3}\\\\\n",
    "    &\\underline{\\text{Number of Addition Terms}} = \\text{Arithmetic Sum} = \\dfrac{n(n+1)}{2}\n",
    "\\end{align*}\n",
    "$$\n",
    "\n",
    "Combined\n",
    "\n",
    "$$\n",
    "\\text{Sum of squares} \\space = \\dfrac{2n + 1}{3} \\cdot \\dfrac{n(n+1)}{2}\n",
    "$$\n",
    "\n",
    "Which is the same as\n",
    "\n",
    "$$\n",
    "\\text{Sum of squares} \\space = \\dfrac{n(n+1)(2n + 1)}{6}\n",
    "$$\n",
    "\n",
    "How Interesting!"
   ]
  },
  {
   "cell_type": "markdown",
   "id": "0b9fad6e-b76e-41a0-934a-fc5220ff832b",
   "metadata": {
    "jp-MarkdownHeadingCollapsed": true
   },
   "source": [
    "# Explore Other Methods (Comprehensive Understanding)\n",
    "\n",
    "To deepen understanding, explore alternative methods:\n",
    "- **Mathematical Induction**: Prove the formula by assuming it holds for $n$ and showing it holds for $n+1$.\n",
    "    - This is a verification approach\n",
    "- **Telescoping Series**: Use $(k+1)^3 - k^3 = 3k^2 + 3k + 1$ to derive the sum.\n",
    "    - This is a top-down derivation approach\n",
    "\n",
    "This comprehensive approach ensures a holistic grasp of the concept."
   ]
  }
 ],
 "metadata": {
  "kernelspec": {
   "display_name": "Python 3 (ipykernel)",
   "language": "python",
   "name": "python3"
  },
  "language_info": {
   "codemirror_mode": {
    "name": "ipython",
    "version": 3
   },
   "file_extension": ".py",
   "mimetype": "text/x-python",
   "name": "python",
   "nbconvert_exporter": "python",
   "pygments_lexer": "ipython3",
   "version": "3.12.9"
  }
 },
 "nbformat": 4,
 "nbformat_minor": 5
}
