{
 "cells": [
  {
   "cell_type": "markdown",
   "id": "c525f452-8e1d-4e50-b106-34f6d498ddf2",
   "metadata": {},
   "source": [
    "# Introduction to Telescoping\n",
    "\n",
    "Let us start from the duality of arithmetics\n",
    "\n",
    "Where we have\n",
    "\n",
    "$$\n",
    "+a \\quad -a\n",
    "$$\n",
    "\n",
    "Every addition $+a$ has its counterpart $-a$ that does the opposite effect\n",
    "- When both are used together, they eliminate each other\n",
    "\n",
    "We can continuously do either of them\n",
    "\n",
    "$$\n",
    "+a \\space +a \\space +a \\space +a \\space +a \\space +a \\cdots\n",
    "$$\n",
    "\n",
    "Or\n",
    "\n",
    "$$\n",
    "-a \\space -a \\space -a \\space -a \\space -a \\space -a \\cdots\n",
    "$$\n",
    "\n",
    "And there is a notation that simplifies this process\n",
    "\n",
    "$$\n",
    "\\sum_{k=1}^{n} +a = \\underbrace{+a \\space +a \\space +a \\space +a \\space +a \\space +a \\cdots + a}_{\\text{n terms}}\n",
    "$$\n",
    "\n",
    "Or\n",
    "\n",
    "$$\n",
    "\\sum_{a=1}^{n} -a = \\underbrace{-a \\space -a \\space -a \\space -a \\space -a \\space -a \\cdots - a}_{\\text{n terms}}\n",
    "$$\n",
    "\n",
    "What if we combine them together during the summation?\n",
    "\n",
    "$$\n",
    "\\sum_{k=1}^{n} +a -a = \\overbrace{\\underbrace{(+a -a)}_{0} \\space \\underbrace{(+a -a)}_{0} \\cdots \\underbrace{(+a -a)}_{0}}^{\\text{n terms}} = 0\n",
    "$$\n",
    "\n",
    "We will just end up with each a bunch of zeros, that amount to nothing.\n",
    "\n",
    "What if we want it to amount to something instead of nothing?"
   ]
  },
  {
   "cell_type": "markdown",
   "id": "97648864-2e32-4857-a414-f7fd753201c0",
   "metadata": {},
   "source": [
    "# Structure of a Summation\n",
    "\n",
    "Lets examine the structure of a summation\n",
    "\n",
    "When we do summation, we have the terms we want to sum\n",
    "\n",
    "- This is if we want to sum the same terms\n",
    "$$\n",
    "\\textcolor{lightgray}{\\sum_{k=1}^{n}} +a\n",
    "$$\n",
    "\n",
    "And we have the starting point `k=1`, and ending point `k=n` of that term\n",
    "\n",
    "$$\n",
    "\\sum_{k=1}^{n} \\textcolor{lightgray}{+a}\n",
    "$$\n",
    "\n",
    "And we also have the `step` of the summation, which is how the start point progresses to the end, by increments of how much?\n",
    "\n",
    "- The step used in summation is the unit step `1`\n",
    "\n",
    "$$\n",
    "1 \\rightarrow 2 \\rightarrow 3 \\rightarrow \\cdots  \\rightarrow n \n",
    "$$"
   ]
  },
  {
   "cell_type": "markdown",
   "id": "9579f9ce-a141-4e7f-981a-b2f4744c798f",
   "metadata": {},
   "source": [
    "# To Amount to Something\n",
    "\n",
    "In order for a summation to amount to something instead of nothing, it must `contain terms that are eliminated`\n",
    "\n",
    "But we have established that in its simplest form, this summation amounts to nothing\n",
    "\n",
    "$$\n",
    "\\sum_{k=1}^n +a -a = 0\n",
    "$$\n",
    "\n",
    "\n",
    "#### Since all terms are generated from the same mold,\n",
    "\n",
    "The only way to eliminate terms without dissolving the entire expression into `0`, is to have \n",
    "- `Terms that are not eliminated`, and thus\n",
    "- Terms that are `eliminated by their later counterparts`.\n",
    "\n",
    "$$\n",
    "\\colorbox{lightgray}{The summation must already contain both `the term to be eliminated` and the `term that will eliminate previous terms`} \n",
    "$$\n",
    "\n",
    "Thus, $+a$ and $-a$ must be `related` in some way\n",
    "\n",
    "$$\n",
    "\\textcolor{lightgray}{\\sum_{k=1}^n} \\boxed{+a} \\longleftrightarrow \\boxed{-a}  \n",
    "$$\n",
    "\n",
    "---\n",
    "\n",
    "How are they related?\n",
    "\n",
    "- It might be hard to imagine what kinds of terms are not eliminated.\n",
    "- But we can think about the `terms that are eliminated by their later counterparts`,\n",
    "\n",
    "What does this mean?\n",
    "\n",
    "It means the current term must be able to match its later counterpart within some steps.\n",
    "\n",
    "### Relationship with Increments\n",
    "\n",
    "- `Matching within some steps` means that it the `terms has to increment`\n",
    "\n",
    "$$\n",
    "\\colorbox{lightgray}{Thus the `terms are related to the increments`}\n",
    "$$\n",
    "\n",
    "$$\n",
    "\\sum_{k=1}^n +k -k\n",
    "$$\n",
    "\n",
    "- `Matching its later counterpart` means its later counterpart must `already be represented in the summation`\n",
    "- And thus related to the `current term` by some relation\n",
    "\n",
    "What is the relation?\n",
    "\n",
    "### Relationship between Terms\n",
    "\n",
    "$$\n",
    "\\colorbox{lightgray}{The later counterpart must be `able to overcome with steps`}\n",
    "$$\n",
    "\n",
    "Which means it must be some multiple of the `steps`\n",
    "\n",
    "Since\n",
    "- `step` is `incremental` and in `integers`,\n",
    "- The difference must be some `positive integer multiple` of the `step`\n",
    "\n",
    "Thus\n",
    "- Let step be `s`, and\n",
    "- `m` be the  multiple of the step, such that $m \\in \\mathbf{Z^{+}}$\n",
    "- Where the difference, `d`, is a `positive integer multiple of s`,\n",
    "    - Such that `d = ms`\n",
    "\n",
    "$$\n",
    "\\sum_{k=1}^n \\underline{+k} \\space -\\underline{(k+ms)}, \\quad \\text{for} \\space m \\in \\mathbf{Z^{+}} \n",
    "$$\n",
    "\n",
    "---\n",
    "\n",
    "And for Summation purposes, the step is `1`\n",
    "- Thus this simplifies\n",
    "\n",
    "$$\n",
    "\\sum_{k=1}^n \\underline{+k} \\space - \\underline{(k+m \\cdot 1)}\n",
    "$$\n",
    "\n",
    "- To this\n",
    "\n",
    "$$\n",
    "\\sum_{k=1}^n \\underline{+k} \\space - \\underline{(k+m)}\n",
    "$$\n",
    "\n",
    "Which means, it is the same as, having the `difference between terms equal to the multiple of the step`,\n",
    "- `d = m`\n",
    "\n",
    "$$\n",
    "\\boxed{\n",
    "    \\sum_{k=1}^n \\underline{+k} \\space - \\underline{(k+d)}, \\quad \\text{for} \\space d \\in \\mathbf{Z^{+}} \n",
    "}\n",
    "$$\n",
    "\n",
    "> Notice that because of a `common difference` that `d` is, the terms in this summation, are also part of an arithmetic series"
   ]
  },
  {
   "cell_type": "markdown",
   "id": "4f079480-32d1-4349-9489-13988e04c72f",
   "metadata": {},
   "source": [
    "# Analyse the Pattern\n",
    "\n",
    "Lets expand it as such as spot for patterns\n",
    "\n",
    "$$\n",
    "\\sum_{k=1}^n \\underline{+k} \\space - \\underline{(k+d)}\n",
    "$$\n",
    "\n",
    "For `d = 3`,\n",
    "\n",
    "$$\n",
    "\\begin{align}\n",
    "    \\sum_{k=1}^n \\underline{+k} \\space - \\underline{(k+3)} &= 1 - \\cancel{4} \\\\\n",
    "    &= 2 - \\cancel{5} \\\\\n",
    "    &= 3 - \\cancel{6} \\\\\n",
    "    &= \\cancel{4} - \\cdots \\\\\n",
    "    &= \\cancel{5} - \\cdots \\\\\n",
    "    &= \\cancel{6} - \\cdots \\\\\n",
    "    &  \\vdots \\\\\n",
    "    &= \\cdots - \\cancel{n-2} \\\\ \n",
    "    &= \\cdots - \\cancel{n-1} \\\\\n",
    "    &= \\cdots - \\cancel{n} \\\\\n",
    "    &= \\cancel{n-2} - (n+1) \\\\ \n",
    "    &= \\cancel{n-1} - (n+2) \\\\\n",
    "    &= \\cancel{n} - (n+3) \\\\\n",
    "\\end{align}\n",
    "$$\n",
    "\n",
    "Notice how the terms in the middle `start to cancel out` once the `increment catches up with the difference` between the terms?\n",
    "\n",
    "The number of terms left is exactly\n",
    "-  `d` amount of the first `smaller terms`\n",
    "    > As they would not have enough increments to start cancelling out the bigger term\n",
    "\n",
    "- And `d` amount of the last `bigger terms`\n",
    "    > As they would have `just enough to not be cancelled out` by the `smaller terms catching up`\n",
    "\n",
    "Thus\n",
    "\n",
    "$$\n",
    "\\sum_{k=1}^n \\underline{+k} \\space - \\underline{(k+d)} = \\text{d amount of the first smaller terms} - \\text{d amount of the last bigger terms} \n",
    "$$\n",
    "\n",
    "Which is\n",
    "\n",
    "$$\n",
    "\\boxed{\n",
    "    \\sum_{k=1}^n \\underline{+k} \\space - \\underline{(k+d)} = \\sum_{k=1}^{d} k - \\sum_{k=(n-d+1)}^n (k+d),  \\quad \\text{for} \\space d \\in \\mathbf{Z^{+}}\n",
    "}\n",
    "$$\n",
    "\n",
    "---\n",
    "\n",
    "Notice that the part containing the last larger terms, can be simplified according to its relationship with the smaller terms\n",
    "\n",
    "$$\n",
    "\\textcolor{lightgray}{\\sum_{k=1}^n \\underline{+k} \\space - \\underline{(k+d)} = \\sum_{k=1}^{d} k \\space - } \\sum_{k=(n-d+1)}^n (k+d) \n",
    "$$\n",
    "\n",
    "- As they are always `d` bigger, they also equal to the summation of the smaller terms extended over `d` range\n",
    "\n",
    "Which in summation presents as the addition of `d` shifting from the terms to the indices\n",
    "\n",
    "$$\n",
    "\\textcolor{lightgray}{\\sum_{k=1}^n \\underline{+k} \\space - \\underline{(k+d)} = \\sum_{k=1}^{d} k \\space - } \\sum_{k=(n-d+1)+d}^{n+d} k \n",
    "$$\n",
    "\n",
    "And thus\n",
    "\n",
    "$$\n",
    "\\textcolor{lightgray}{\\sum_{k=1}^n \\underline{+k} \\space - \\underline{(k+d)} = \\sum_{k=1}^{d} k \\space - } \\sum_{k=n+1}^{n+d} k \n",
    "$$\n",
    "\n",
    "Thus, we have the simplified formula of\n",
    "\n",
    "$$\n",
    "\\boxed{\n",
    "    \\sum_{k=1}^n \\underline{+k} \\space - \\underline{(k+d)} = \\sum_{k=1}^{d} k \\space - \\sum_{k=n+1}^{n+d} k,  \\quad \\text{for} \\space d \\in \\mathbf{Z^{+}} \n",
    "}\n",
    "$$\n",
    "\n"
   ]
  },
  {
   "cell_type": "markdown",
   "id": "aa00b1ac-2772-48b1-80d8-6fe74e1815ab",
   "metadata": {},
   "source": [
    "# The Simple Case\n",
    "\n",
    "Notice that in the previous case, we set `d` to `3` to show how it cancels out\n",
    "\n",
    "$$\n",
    "\\begin{align}\n",
    "    \\sum_{k=1}^n \\underline{+k} \\space - \\underline{(k+3)} &= 1 - \\cancel{4} \\\\\n",
    "    &= 2 - \\cancel{5} \\\\\n",
    "    &= 3 - \\cancel{6} \\\\\n",
    "    &= \\cancel{4} - \\cdots \\\\\n",
    "    &= \\cancel{5} - \\cdots \\\\\n",
    "    &= \\cancel{6} - \\cdots \\\\\n",
    "    &  \\vdots \\\\\n",
    "    &= \\cdots - \\cancel{n-2} \\\\ \n",
    "    &= \\cdots - \\cancel{n-1} \\\\\n",
    "    &= \\cdots - \\cancel{n} \\\\\n",
    "    &= \\cancel{n-2} - (n+1) \\\\ \n",
    "    &= \\cancel{n-1} - (n+2) \\\\\n",
    "    &= \\cancel{n} - (n+3) \\\\\n",
    "\\end{align}\n",
    "$$\n",
    "\n",
    "Notice that if we shrink `d` to `1`, this happens\n",
    "\n",
    "$$\n",
    "\\begin{align}\n",
    "    \\sum_{k=1}^n \\underline{+k} \\space - \\underline{(k+1)} &= 1 - \\cancel{2} \\\\\n",
    "    &= \\cancel{2} - \\cancel{3} \\\\\n",
    "    &= \\cancel{3} - \\cancel{4} \\\\\n",
    "    &= \\cancel{4} - \\cdots \\\\\n",
    "    &  \\vdots \\\\\n",
    "    &= \\cdots - \\cancel{n-1} \\\\\n",
    "    &= \\cancel{n-1} - \\cancel{n} \\\\\n",
    "    &= \\cancel{n} - (n+1) \\\\\n",
    "\\end{align}\n",
    "$$\n",
    "\n",
    "We are left with just the `first smaller term`, and the `last bigger term`\n",
    "- This is because with a difference, `d`, of only `1`, the next iteration already caught up with the difference\n",
    "- Which causes direct elimination on iteration right after the first\n",
    "\n",
    "Thus, we can simplify this case where `d=1`, from the formula as well\n",
    "\n",
    "- From the formula\n",
    "\n",
    "$$\n",
    "\\sum_{k=1}^n \\underline{+k} \\space - \\underline{(k+d)} = \\sum_{k=1}^{d} k \\space - \\sum_{k=n+1}^{n+d} k \n",
    "$$\n",
    "\n",
    "- Let `d=1`\n",
    "\n",
    "$$\n",
    "\\begin{align}\n",
    "    \\sum_{k=1}^n \\underline{+k} \\space - \\underline{(k+\\boxed{1})} &= \\sum_{k=1}^{\\boxed{1}} k \\space - \\sum_{k=n+1}^{n+\\boxed{1}} k \\\\\n",
    "    &= \\underline{\\text{1st term}} - \\underline{\\text{(n+1)-th term}} \\\\\n",
    "    &= k_{1} - k_{n+1}\n",
    "\\end{align}\n",
    "$$\n",
    "\n",
    "And Thus, we can also see that we arrived at the same conclusion\n",
    "\n",
    "$$\n",
    "\\boxed{\n",
    "    \\sum_{k=1}^n \\underline{+k} \\space - \\underline{(k+1)} = k_{1} - k_{n+1} \n",
    "}\n",
    "$$\n",
    "\n",
    "Of course the direct answer here is `-n`, but we are looking for patterns, not just direct answers"
   ]
  },
  {
   "cell_type": "markdown",
   "id": "4a4764fc-9c85-402f-a275-9a711d6cb780",
   "metadata": {},
   "source": [
    "# For all Transformations\n",
    "\n",
    "Thus, from the above, we concluded that as long as the `2 terms` are `related in difference` that is a `positive multiple of the step`, `(which is an incrementing positive integer)`, the step will be able to `catch up with the difference`\n",
    "\n",
    "---\n",
    "\n",
    "- Where `d = ms`\n",
    "\n",
    "$$\n",
    "\\sum_{k=1}^n \\underline{+k} \\space - \\underline{(k+d)}, \\quad \\text{for} \\space d \\in \\mathbf{Z^{+}} \n",
    "$$\n",
    "\n",
    "- Causing `later terms cancel out previous terms`, which `simplifies the sum`\n",
    "\n",
    "$$\n",
    "\\sum_{k=1}^n \\underline{+k} \\space - \\underline{(k+d)} = \\sum_{k=1}^{d} k \\space - \\sum_{k=n+1}^{n+d} k, \\quad \\text{for} \\space d \\in \\mathbf{Z^{+}} \n",
    "$$\n",
    "\n",
    "- And with the special case\n",
    "\n",
    "$$\n",
    "\\sum_{k=1}^n \\underline{+k} \\space - \\underline{(k+1)} = k_{1} - k_{n+1} \n",
    "$$\n",
    "\n",
    "---\n",
    "\n",
    "With this in mind, \n",
    "\n",
    "#### Any unique transformation of those 2 terms, as long as it is the same transformation, will be able to carry over these properties.\n",
    "\n",
    "And what things transform uniquely? \n",
    "> Functions!\n",
    "\n",
    "Thus, with functions, we carry over the same properties of the `step catching up with the difference`\n",
    "\n",
    "$$\n",
    "\\boxed{\n",
    "    \\text{Telescoping Sum} \\space = \\space \\sum_{k=1}^n \\underline{f(k)} - \\underline{f(k+d)}, \\quad \\text{for} \\space d \\in \\mathbf{Z^{+}}\n",
    "}\n",
    "$$\n",
    "\n",
    "Which means, undergoing the same derivations, this works\n",
    "\n",
    "$$\n",
    "\\boxed{\n",
    "    \\sum_{k=1}^n \\underline{f(k)} - \\underline{f(k+d)} = \\sum_{k=1}^{d} f(k) \\space - \\sum_{k=n+1}^{n+d} f(k), \\quad \\text{for} \\space d \\in \\mathbf{Z^{+}}\n",
    "}\n",
    "$$\n",
    "\n",
    "- Note that the above works, whether or not `step = 1`\n",
    "\n",
    "And the special case where `d=1`, works too\n",
    "\n",
    "$$\n",
    "\\boxed{\n",
    "    \\sum_{k=1}^n \\underline{f(k)} - \\underline{f(k+1)} = f(1) - f(n+1) \n",
    "}\n",
    "$$\n",
    "\n",
    "> Those are thus the General Form of Telescoping Sums"
   ]
  },
  {
   "cell_type": "markdown",
   "id": "d374bef3-251a-44be-8fde-4c2a0ac74230",
   "metadata": {},
   "source": [
    "# Telescoping Products from Telescoping Sums\n",
    "\n",
    "With this knowledge we can also expand it to Telescoping Products. \n",
    "\n",
    "\n",
    "Since the telescoping properties only depend on \n",
    "- The `2 terms`, for which they have `operations inverse of each other`, that match the `repeated operator`\n",
    "    - i.e. `For Summation: add/subtract, For Product: multiply/divide`\n",
    "- The difference between those 2 terms is a `positive multiple` of the step\n",
    "\n",
    "Then we have\n",
    "- Where `d = ms`\n",
    "\n",
    "\n",
    "$$\n",
    "\\prod_{k=1}^n \\dfrac{k}{k+d}, \\quad \\text{for} \\space d \\in \\mathbf{Z^{+}}\n",
    "$$\n",
    "\n",
    "Thus, with the same logic, for lets say `d = 2`\n",
    "\n",
    "$$\n",
    "\\prod_{k=1}^n \\dfrac{k}{k+d} = \\dfrac{1}{\\cancel{3}} \\cdot \\dfrac{2}{\\cancel{4}} \\cdot \\dfrac{\\cancel{3}}{\\cdots} \\cdot \\dfrac{\\cancel{4}}{\\cdots} \\cdots \\dfrac{\\cdots}{\\cancel{n-1}} \\dfrac{\\cdots}{\\cancel{n}} \\cdot \\dfrac{\\cancel{n-1}}{n+1} \\cdot \\dfrac{\\cancel{n}}{n+2} \n",
    "$$\n",
    "\n",
    "We can arrive at the general formula\n",
    "\n",
    "$$\n",
    "\\prod_{k=1}^n \\dfrac{k}{k+d} = \\dfrac{\\prod_{k=1}^{d} k}{\\prod_{k=n+1}^{n+d} k}, \\quad \\text{for} \\space d \\in \\mathbf{Z^{+}}\n",
    "$$\n",
    "\n",
    "And its special case\n",
    "\n",
    "$$\n",
    "\\prod_{k=1}^n \\dfrac{k}{k+1} = \\dfrac{1}{n+1}\n",
    "$$\n",
    "\n",
    "For which, any unique transformation of that property, will retain the properties of telescoping.\n",
    "\n",
    "\n",
    "$$\n",
    "\\boxed{\n",
    "    \\text{Telescoping Product} \\space = \\space \\prod_{k=1}^n \\dfrac{f(k)}{f(k+d)}, \\quad \\text{for} \\space d \\in \\mathbf{Z^{+}}\n",
    "}\n",
    "$$\n",
    "\n",
    "Such that\n",
    "\n",
    "$$\n",
    "\\boxed{\n",
    "    \\prod_{k=1}^n \\dfrac{f(k)}{f(k+d)} = \\dfrac{\\prod_{k=1}^{d} f(k)}{\\prod_{k=n+1}^{n+d} f(k)}, \\quad \\text{for} \\space d \\in \\mathbf{Z^{+}}\n",
    "}\n",
    "$$\n",
    "\n",
    "And its special case\n",
    "\n",
    "$$\n",
    "\\boxed{\n",
    "    \\prod_{k=1}^n \\dfrac{f(k)}{f(k+1)} = \\dfrac{f(1)}{f(n+1)}\n",
    "}\n",
    "$$"
   ]
  },
  {
   "cell_type": "markdown",
   "id": "0fec5ebc-d98c-4251-811f-9cd29af6b7fe",
   "metadata": {},
   "source": [
    "# Conclusion\n",
    "\n",
    "Thus! Since, any expression in repeated operator such that\n",
    "- The input of the `2 terms` are related by a `positive multiple` of the step of the repeated operator i.e. `Summation/Product`\n",
    "- And their `inverse operations` are exactly `the same as` that of the repeated operator\n",
    "\n",
    "You can get a definite simplified answer by expressing some expressions in these forms\n",
    "\n",
    "---\n",
    "\n",
    "- Where `d = ms`\n",
    "\n",
    "#### Telescoping Sum\n",
    "$$\n",
    "\\boxed{\n",
    "    \\sum_{k=1}^n \\underline{f(k)} - \\underline{f(k+d)} = \\sum_{k=1}^{d} f(k) \\space - \\sum_{k=n+1}^{n+d} f(k), \\quad \\text{for} \\space d \\in \\mathbf{Z^{+}}\n",
    "}\n",
    "$$\n",
    "\n",
    "#### Telescoping Product\n",
    "$$\n",
    "\\boxed{\n",
    "    \\prod_{k=1}^n \\dfrac{f(k)}{f(k+d)} = \\dfrac{\\prod_{k=1}^{d} f(k)}{\\prod_{k=n+1}^{n+d} f(k)}, \\quad \\text{for} \\space d \\in \\mathbf{Z^{+}}\n",
    "}\n",
    "$$"
   ]
  },
  {
   "cell_type": "markdown",
   "id": "10ea96b6-b00f-4c1a-bb27-2f2940f586d6",
   "metadata": {},
   "source": [
    "# Table of Reference\n",
    "\n",
    "---\n",
    "\n",
    "# Sums\n",
    "\n",
    "$$\n",
    "\\begin{array}{c|c|c}\n",
    "\\hline\n",
    "\\quad \\textbf{Step Difference } (d) & \\textbf{Surviving Terms} & \\textbf{Simplified Result} \\\\\n",
    "\\hline\n",
    "1 & f(1), f(n+1) & f(1) - f(n+1) \\\\\n",
    "2 & f(1), f(2), f(n+1), f(n+2) & f(1) + f(2) - f(n+1) - f(n+2) \\\\\n",
    "3 & f(1), f(2), f(3), f(n+1), f(n+2), f(n+3) & f(1) + f(2) + f(3) - f(n+1) - f(n+2) - f(n+3) \\\\\n",
    "\\vdots & \\vdots & \\vdots \\\\\n",
    "d & \\sum_{k=1}^{d} f(k), \\sum_{k=n+1}^{n+d} f(k) & \\sum_{k=1}^{d} f(k) - \\sum_{k=n+1}^{n+d} f(k) \\\\\n",
    "\\hline\n",
    "\\end{array}\n",
    "$$\n",
    "\n",
    "\n",
    "# Products\n",
    "\n",
    "$$\n",
    "\\begin{array}{c|c|c}\n",
    "\\hline\n",
    "\\quad \\textbf{Step Difference } (d) & \\textbf{Surviving Terms} & \\textbf{Simplified Result} \\\\\n",
    "\\hline\n",
    "1 & f(1), f(n+1) & \\displaystyle \\frac{f(1)}{f(n+1)} \\\\\n",
    "2 & f(1), f(2), f(n+1), f(n+2) & \\displaystyle \\frac{f(1) \\cdot f(2)}{f(n+1) \\cdot f(n+2)} \\\\\n",
    "3 & f(1), f(2), f(3), f(n+1), f(n+2), f(n+3) & \\displaystyle \\frac{f(1) \\cdot f(2) \\cdot f(3)}{f(n+1) \\cdot f(n+2) \\cdot f(n+3)} \\\\\n",
    "\\vdots & \\vdots & \\vdots \\\\\n",
    "d & \\prod_{k=1}^{d} f(k), \\prod_{k=n+1}^{n+d} f(k) & \\displaystyle \\frac{\\prod_{k=1}^{d} f(k)}{\\prod_{k=n+1}^{n+d} f(k)} \\\\\n",
    "\\hline\n",
    "\\end{array}\n",
    "$$"
   ]
  }
 ],
 "metadata": {
  "kernelspec": {
   "display_name": "Python 3 (ipykernel)",
   "language": "python",
   "name": "python3"
  },
  "language_info": {
   "codemirror_mode": {
    "name": "ipython",
    "version": 3
   },
   "file_extension": ".py",
   "mimetype": "text/x-python",
   "name": "python",
   "nbconvert_exporter": "python",
   "pygments_lexer": "ipython3",
   "version": "3.12.9"
  }
 },
 "nbformat": 4,
 "nbformat_minor": 5
}
