{
 "cells": [
  {
   "cell_type": "markdown",
   "id": "7ba3f499-f425-48f3-bb92-0ff7b62b401a",
   "metadata": {},
   "source": [
    "# Combinatorial Approach to the Sum of Squares Formula\n",
    "\n",
    "We derive the formula for the sum of squares using a combinatorial approach by expressing the sum as a double summation, applying the arithmetic sequence formula, and then using algebraic manipulation.\n",
    "\n",
    "---"
   ]
  },
  {
   "cell_type": "markdown",
   "id": "fe7e0630-ade2-4eed-b0f9-c9fc218cd7ef",
   "metadata": {},
   "source": [
    "## Transforming the Sum into a Familiar Form\n",
    "\n",
    "With a bit of play, we can break the sum of $\\sum_{k=1}^n k^2$ like this:\n",
    "\n",
    "$$\n",
    "\\sum_{k=1}^n k^2 = 1^2 + 2^2 + 3^2 + ... + n^2\n",
    "$$\n",
    "\n",
    "$$\n",
    "\\sum_{k=1}^n k^2 = (1 \\cdot 1) + (2 \\cdot 2) + (3 \\cdot 3) + ... + (n \\cdot n)\n",
    "$$\n",
    "\n",
    "$$\n",
    "\\sum_{k=1}^n k^2 = 1 + (2 + 2) + (3 + 3 + 3) + ... + (\\underbrace{n + n + \\dots + n}_{n \\text{ times}})\n",
    "$$\n",
    "\n",
    "$$\n",
    "\\sum_{k=1}^n k^2 = \\underbrace{(1 + 2 + 3 + ... + n) + (2 + 3 + 4 + ... + n) + ... + n}_{n \\text{ terms}}\n",
    "$$\n",
    "\n",
    "$$\n",
    "\\sum_{k=1}^n k^2 = \\underbrace{\\sum_{j=1}^n j + \\sum_{j=2}^n j + ... + \\sum_{j=n}^n j}_{n \\text{ terms}}\n",
    "$$\n",
    "\n",
    "And thus we get this Double Summation:\n",
    "\n",
    "$$\n",
    "\\boxed{\\sum_{k=1}^n k^2 = \\sum_{k=1}^n \\sum_{j=k}^{n} j}\n",
    "$$\n",
    "\n",
    "---\n",
    "\n",
    "## Visualising the Sum in 2 Dimensions\n",
    "\n",
    "We can also visualise this transformation much more distinctly by setting the terms up in a 2-dimensional form:\n",
    "\n",
    "$$\n",
    "\\begin{array}{c|ccccc}\n",
    "    & j=1 & j=2 & j=3 & \\cdots & \\cdots & \\cdots & j=n \\\\\n",
    "\\hline\n",
    "    k=1 & 1 \\\\\n",
    "    k=2 & 2 & 2 \\\\\n",
    "    k=3 & 3 & 3 & 3 \\\\\n",
    "    k=4 & 4 & 4 & 4 & 4 \\\\\n",
    "    k=5 & 5 & 5 & 5 & 5 & 5 \\\\\n",
    "    \\vdots & \\vdots & \\vdots & \\vdots & \\vdots & \\vdots & \\ddots \\\\\n",
    "    k=n & n & n & n & n & n & \\cdots & n \\\\\n",
    "\\hline\n",
    "    \\text{Sum} & \\sum_{i=1}^{n} i & \\sum_{i=2}^{n} i & \\sum_{i=3}^{n} i & \\sum_{i=4}^{n} i & \\sum_{i=5}^{n} i & \\cdots & \\sum_{i=n}^{n} i\n",
    "\\end{array}\n",
    "$$\n",
    "\n",
    "By arranging it like this, we can realise that although we can sum it the way we were told, left-right then top-down, it can be expressed equally as well in Summation Notation:\n",
    "\n",
    "$$\n",
    "\\sum_{\\text{row } k=1}^{n} (\\text{sum of row } k) = \\sum_{k=1}^{n} \\sum_{m=1}^{j} j = \\sum_{k=1}^{n} (j \\times j) = \\sum_{k=1}^{n} i^2\n",
    "$$\n",
    "\n",
    "We can notice that we can also sum it in terms of arithmetic sequences as seen if we choose to follow the sum top-down then left-right.\n",
    "\n",
    "$$\n",
    "\\sum_{k=1}^n k^2 = \\sum_{k=1}^{n} \\sum_{j=k}^{n} j\n",
    "$$\n",
    "\n",
    "And thus we get this Double Summation:\n",
    "\n",
    "$$\n",
    "\\boxed{\\sum_{k=1}^n k^2 = \\sum_{k=1}^{n} \\sum_{j=k}^{n} j}\n",
    "$$"
   ]
  },
  {
   "cell_type": "markdown",
   "id": "7c7e81de-c151-4a83-b15c-b7aaf5dc4765",
   "metadata": {},
   "source": [
    "## Apply the Arithmetic Sequence Formula\n",
    "\n",
    "Let\n",
    "$$\n",
    "\\mathbf{S} = \\sum_{k=1}^n k^2 = \\sum_{k=1}^{n} \\sum_{j=k}^{n} j\n",
    "$$\n",
    "\n",
    "The inner sum $\\sum_{i=k}^n i$ is an arithmetic sequence with:\n",
    "- First term: $k$\n",
    "- Last term: $n$\n",
    "- Number of terms: $n - k + 1$\n",
    "\n",
    "The sum of an arithmetic sequence is:\n",
    "\n",
    "$$\n",
    "\\left( \n",
    "    \\dfrac{\\text{first term} + \\text{last term}}{2} \n",
    "\\right) (\\text{number of terms})\n",
    "$$\n",
    "\n",
    "$$\n",
    "\\left( \n",
    "    \\dfrac{n + k}{2} \n",
    "\\right) (n - k + 1)\n",
    "$$\n",
    "\n",
    "Thus:\n",
    "\n",
    "$$\n",
    "\\sum_{k=1}^n \\dfrac{(n + k)(n - k + 1)}{2}\n",
    "$$\n",
    "\n",
    "Factor out $\\dfrac{1}{2}$:\n",
    "\n",
    "$$\n",
    "\\dfrac{1}{2} \\sum_{k=1}^n (n + k)(n - k + 1)\n",
    "$$\n",
    "\n",
    "---\n",
    "\n",
    "## Simplify the Inner Expression\n",
    "\n",
    "Expand the inner expression $(n + k)(n - k + 1)$:\n",
    "\n",
    "$$\n",
    "\\begin{aligned}\n",
    "    (n + k)(n - k + 1) &= n^2 - nk + n + kn - k^2 + k \\\\\n",
    "                       &= n^2 + n - k^2 + k\n",
    "\\end{aligned}\n",
    "$$\n",
    "\n",
    "Substitute back into the sum:\n",
    "\n",
    "$$\n",
    "\\dfrac{1}{2} \\sum_{k=1}^n (n^2 + n - k^2 + k)\n",
    "$$\n",
    "\n",
    "Break into individual sums:\n",
    "\n",
    "$$\n",
    "\\dfrac{1}{2} \n",
    "\\left( \n",
    "    \\sum_{k=1}^n n^2 + \\sum_{k=1}^n n - \\sum_{k=1}^n k^2 + \\sum_{k=1}^n k \n",
    "\\right)\n",
    "$$\n",
    "\n",
    "Simplify:\n",
    "\n",
    "$$\n",
    "\\dfrac{1}{2} \n",
    "\\left[ \n",
    "    n^3 + n^2 - \\mathbf{S} + \\dfrac{n(n+1)}{2} \n",
    "\\right]\n",
    "$$\n",
    "\n",
    "Balance the equation:\n",
    "\n",
    "$$\n",
    "\\mathbf{S} = \\dfrac{1}{2} \\left[\n",
    "    n^3 + n^2 - \\mathbf{S} + \\dfrac{n(n+1)}{2} \n",
    "\\right]\n",
    "$$\n",
    "\n",
    "$$\n",
    "2\\mathbf{S} = n^3 + n^2 - \\mathbf{S} + \\dfrac{n(n+1)}{2}\n",
    "$$\n",
    "\n",
    "$$\n",
    "3\\mathbf{S} = n^3 + n^2 + \\dfrac{n(n+1)}{2}\n",
    "$$\n",
    "\n",
    "$$\n",
    "3\\mathbf{S} = \\dfrac{2n^3 + 2n^2 + n^2 + n}{2}\n",
    "$$\n",
    "\n",
    "$$\n",
    "\\begin{aligned}\n",
    "    \\mathbf{S} &= \\dfrac{2n(n^2 + n) + (n^2 + n)}{6} \\\\\n",
    "    \\mathbf{S} &= \\dfrac{(n^2 + n)(2n + 1)}{6} \\\\\n",
    "    \\mathbf{S} &= \\dfrac{n(n + 1)(2n + 1)}{6}\n",
    "\\end{aligned}\n",
    "$$\n",
    "\n",
    "Therefore:\n",
    "\n",
    "$$\n",
    "\\boxed{ \\sum_{k=1}^n k^2 = \\dfrac{n(n + 1)(2n + 1)}{6} }\n",
    "$$"
   ]
  },
  {
   "cell_type": "markdown",
   "id": "fd758ac0-2b57-47c8-af1d-6f5d042a199f",
   "metadata": {},
   "source": [
    "## Additional Insights\n",
    "From this we can see that also:\n",
    "\n",
    "$$\n",
    "\\sum_{k=1}^n k^2 = \\left( \\dfrac{2n + 1}{3} \\right) \\left[ \\dfrac{n(n + 1)}{2} \\right]\n",
    "$$\n",
    "\n",
    "$$\n",
    "\\sum_{k=1}^n k^2 = \\left( \\dfrac{2n + 1}{3} \\right) \\sum_{k=1}^n k\n",
    "$$\n",
    "\n",
    "\n",
    "Therefore, the sum of squares is connected to the common arithmetic sum by a factor of $ \\frac{2n + 1}{3} $"
   ]
  },
  {
   "cell_type": "markdown",
   "id": "25ab6dc1-afbe-4af8-8ffa-9f0cffbb8bd4",
   "metadata": {},
   "source": [
    "---"
   ]
  },
  {
   "cell_type": "markdown",
   "id": "0b9fad6e-b76e-41a0-934a-fc5220ff832b",
   "metadata": {
    "jp-MarkdownHeadingCollapsed": true
   },
   "source": [
    "## Explore Other Methods (Comprehensive Understanding)\n",
    "\n",
    "To deepen understanding, explore alternative methods:\n",
    "- **Mathematical Induction**: Prove the formula by assuming it holds for $n$ and showing it holds for $n+1$.\n",
    "- **Telescoping Series**: Use $(k+1)^3 - k^3 = 3k^2 + 3k + 1$ to derive the sum.\n",
    "\n",
    "This comprehensive approach ensures a holistic grasp of the concept."
   ]
  }
 ],
 "metadata": {
  "kernelspec": {
   "display_name": "Python 3 (ipykernel)",
   "language": "python",
   "name": "python3"
  },
  "language_info": {
   "codemirror_mode": {
    "name": "ipython",
    "version": 3
   },
   "file_extension": ".py",
   "mimetype": "text/x-python",
   "name": "python",
   "nbconvert_exporter": "python",
   "pygments_lexer": "ipython3",
   "version": "3.12.9"
  }
 },
 "nbformat": 4,
 "nbformat_minor": 5
}
